Some missing theorems added. For instance, "parallel_steady_state_avail"..

AvailabilityScript.sml
@@ -1,33 +1,35 @@
 (* ========================================================================= *)
-(* File Name: Availability.sml		                                     *)
+(* File Name: Availability.sml		                                     	 *)
 (*---------------------------------------------------------------------------*)
 (* Description: Formal Availability Analysis using Theorem Proving           *)
-(*                   				                             *)
+(*                   				                                         *)
 (*                                                                           *)
-(*                HOL4-Kananaskis 10 		 			     *)
-(*									     *)
-(*		Author :  Waqar Ahmed             		     	     *)
-(*                                              			     *)
-(* 	    School of Electrical Engineering and Computer Sciences (SEECS)   *)
-(*	    National University of Sciences and Technology (NUST), PAKISTAN  *)
-(*                                          		               	     *)
+(*                HOL4-Kananaskis 10 		 			      				 *)
+(*									     									 *)
+(*		Author :  Waqar Ahmed             		     	     				 *)
+(*                                              			     			 *)
+(* 	    School of Electrical Engineering and Computer Sciences (SEECS)   	 *)
+(*	    National University of Sciences and Technology (NUST), PAKISTAN  	 *)
+(*                                          		               	     	 *)
 (*                                                                           *)
 (* ========================================================================= *)
 
 
+
+
+
+
+
 app load ["arithmeticTheory", "realTheory", "prim_recTheory", "seqTheory",
-    	  "pred_setTheory","res_quanTheory", "res_quanTools", "listTheory", 
-	  "probabilityTheory", "numTheory", "transcTheory", "rich_listTheory", 
-	  "pairTheory","combinTheory","limTheory","sortingTheory", "realLib", 
-	  "optionTheory","satTheory","util_probTheory", "extrealTheory", 
-	  "measureTheory", "lebesgueTheory","real_sigmaTheory","dep_rewrite",
-	  "RBDTheory","FT_deepTheory","VDCTheory","transform_FT_RBDTheory"];
-open HolKernel Parse boolLib bossLib limTheory arithmeticTheory realTheory 
-     prim_recTheory probabilityTheory seqTheory pred_setTheory res_quanTheory 
-     sortingTheory res_quanTools listTheory transcTheory rich_listTheory pairTheory 
-     combinTheory realLib  optionTheory util_probTheory extrealTheory measureTheory 
-     lebesgueTheory real_sigmaTheory satTheory numTheory dep_rewrite 
-     RBDTheory FT_deepTheory VDCTheory transform_FT_RBDTheory;
+    	  "pred_setTheory","res_quanTheory", "res_quanTools", "listTheory", "probabilityTheory", "numTheory",
+	  "transcTheory", "rich_listTheory", "pairTheory",
+	  "combinTheory","limTheory","sortingTheory", "realLib", "optionTheory","satTheory",
+	  "util_probTheory", "extrealTheory", "measureTheory", "lebesgueTheory","real_sigmaTheory","dep_rewrite","RBDTheory","FT_deepTheory","VDCTheory"];
+open HolKernel Parse boolLib bossLib limTheory arithmeticTheory realTheory prim_recTheory probabilityTheory 
+     seqTheory pred_setTheory res_quanTheory sortingTheory res_quanTools listTheory transcTheory
+     rich_listTheory pairTheory combinTheory realLib  optionTheory
+      util_probTheory extrealTheory measureTheory lebesgueTheory real_sigmaTheory satTheory numTheory dep_rewrite 
+      RBDTheory FT_deepTheory VDCTheory;
 
 fun K_TAC _ = ALL_TAC;
 
@@ -160,12 +162,12 @@ val expec_avail1_def = Define
 val cdf_def = Define `cdf p X t = distribution p X {y| y <= t} `;
 
 (*---------------------------------*)
-val rel_event_def = Define `rel_event1 p X t = PREIMAGE X {y | t < y} INTER p_space p`;
-
-(*---------------------------------*)
 val reliability_def = Define 
 `reliability p X t = 1 - cdf p X t `;
 
+
+(*---------------------------------*)
+val rel_event_def = Define `rel_event1 p X t = PREIMAGE X {y | t < y} INTER p_space p`;
 (*-------------------------*)
 val expec_def = Define 
 `expec n f = sum (0,n) f`;
@@ -237,7 +239,11 @@ val two_dim_steady_state_avail_prod_def = Define
 `(two_dim_steady_state_avail_prod [] = (1:real)) /\ 
  (two_dim_steady_state_avail_prod (h::t) =  
   steady_state_avail_prod h * two_dim_steady_state_avail_prod t)`;
-
+(*-----------------------------------*)
+val compl_steady_state_avail_def = Define 
+`(compl_steady_state_avail [] = 1) /\
+ (compl_steady_state_avail (h::t) = 
+ (1 - steady_state_avail h) * compl_steady_state_avail (t))`;
 (*---------------------------------*)
 val compl_rel_event_eq_fail_events = store_thm("compl_rel_event_eq_fail_event1",
   ``!p t s. prob_space p ==> 
@@ -252,8 +258,10 @@ val compl_fail_event_eq_rel_event1 = store_thm("compl_fail_event_eq_rel_event1",
   RW_TAC std_ss[rel_event_def]
   ++ SRW_TAC[][IN_DIFF,PREIMAGE_def,EXTENSION,GSPECIFICATION]
   ++ RW_TAC std_ss[GSYM extreal_lt_def]
-  ++ METIS_TAC[]);
+  ++ METIS_TAC[]); 
 (*--------------------------------*)
+
+(*---------------------------------*)
 val avail_ge_rel = store_thm("avail_ge_rel",
   ``!p t L. 
         (0 ≤ t) /\
@@ -327,8 +335,7 @@ val avail_ge_rel1 = store_thm("avail_ge_rel1",
          ((reliability p (FST (HD L)) (Normal t)) <=
 	  prob p (union_avail_events L (LENGTH L) (t)))  ``,
 RW_TAC std_ss[]
-++ (`prob p (union_avail_events L (LENGTH L) t) = 
-     sum (0,LENGTH L) (prob p o (\a. avail_event L a (Normal t)))`  by MATCH_MP_TAC EQ_SYM)
+++ (`prob p (union_avail_events L (LENGTH L) t) = sum (0,LENGTH L) (prob p o (\a. avail_event L a (Normal t)))`  by MATCH_MP_TAC EQ_SYM)
 >> (MATCH_MP_TAC PROB_FINITELY_ADDITIVE
    ++ RW_TAC std_ss[]
    ++ RW_TAC std_ss[union_avail_events_def]
@@ -340,6 +347,8 @@ RW_TAC std_ss[]
 ++ RW_TAC real_ss[]
 ++ FULL_SIMP_TAC list_ss[IN_COUNT]);
 
+
+(*-------------------------------*)
 (*-------------------------neg_exp_tend0_new-------------------------------------------*)
 val neg_exp_tend0_new = store_thm("neg_exp_tend0_new",
   ``!t (c:real). (0 < c) ==> (\t. exp (&t*(-c)))--> 0``,
@@ -377,9 +386,7 @@ REAL_ARITH_TAC);
 
 (*---------------------------------------------*)
 val steady_state_avail = store_thm("steady_state_avail",
-  ``!p L n m t.  
-       ((0 < FST m) /\ (0 < SND m)) /\ inst_avail_exp p L n m ==> 
-        (lim(\t.  (expec_avail p L n (Normal &t))) = SND m / (SND m + FST m))``,
+  ``!p L n m t.  ((0 < FST m)/\ (0 < SND m)) /\ inst_avail_exp p L n m ==> (lim(\t.  (expec_avail p L n (Normal &t))) = SND m / (SND m + FST m))``,
 RW_TAC std_ss[]
 ++ MATCH_MP_TAC SEQ_UNIQ
 ++ EXISTS_TAC (--`((\t. expec_avail p L n (Normal &t)))`--)
@@ -456,8 +463,7 @@ val steady_state_avail1 = store_thm("steady_state_avail1",
 		       (prob p (union_avail_events L n (&t)))) = 
 		 SND m / (SND m + FST m))``,
 RW_TAC std_ss[]
-++ (`!t. prob p (union_avail_events L n t) = 
-   	 sum (0,n) (prob p o (\a. avail_event L a (Normal t)))`  by RW_TAC std_ss[])
+++ (`!t. prob p (union_avail_events L n t) = sum (0,n) (prob p o (\a. avail_event L a (Normal t)))`  by RW_TAC std_ss[])
 >> (MATCH_MP_TAC EQ_SYM
    ++ MATCH_MP_TAC PROB_FINITELY_ADDITIVE
    ++ RW_TAC std_ss[]
@@ -501,6 +507,9 @@ RW_TAC std_ss[extreal_not_le]);
 val not_null_leng = store_thm("not_null_leng",
   ``! L1 . ~NULL L1  ==> 1 <= LENGTH L1``,
 FULL_SIMP_TAC list_ss[GSYM LENGTH_NOT_NULL]);
+
+(*---------------------------*)
+
 (*----------------------------*)
 val series_expec_tends_prod_avail = store_thm("series_expec_tends_prod_avail",
   ``!p L M. 
@@ -520,15 +529,15 @@ GEN_TAC
 ++ Induct
 >> (RW_TAC list_ss[])
 ++  RW_TAC list_ss[union_avail_event_list1_def,list_prod_def,list_prob_def,steady_state_avail_prod_def] 
-++ (`!t. (prob p (union_avail_events1 h (&t)) *
+++ (`!t. (
+   prob p (union_avail_events1 h (&t)) *
    list_prod
      (list_prob p
-        (MAP (\a. union_avail_events1 a (&t)) L))) = 
-      (\t.
-	prob p (union_avail_events1 h (&t))) t *
-   	(\t. list_prod
-		(list_prob p
-        		   (MAP (\a. union_avail_events1 a (&t)) L))) t` by RW_TAC real_ss[])
+        (MAP (\a. union_avail_events1 a (&t)) L))) = (\t.
+   prob p (union_avail_events1 h (&t))) t *
+   (\t. list_prod
+     (list_prob p
+        (MAP (\a. union_avail_events1 a (&t)) L))) t` by RW_TAC real_ss[])
 ++ POP_ORW
 ++ MATCH_MP_TAC SEQ_MUL
 ++ RW_TAC std_ss[]
@@ -536,20 +545,14 @@ GEN_TAC
    ++ REWRITE_TAC[steady_state_avail_def]
    ++ (`((\t.
      SND (h':real#real) / (SND h' + FST h') +
-     FST h' / (SND h' + FST h') * exp (-(SND h' + FST h') * &t)) --> 
-     (SND h' / (SND h' + FST h'))) = 
-     ((\t.
-	(\t. SND h' / (SND  h'+ FST h')) t +
-     	(\t. FST h' / (SND h' + FST h') * exp (-(SND h' + FST h') * &t))t) --> 
-	(SND h' / (SND h' + FST h') + 0))` by RW_TAC real_ss[])
+     FST h' / (SND h' + FST h') * exp (-(SND h' + FST h') * &t))--> (SND h' / (SND h' + FST h'))) = ((\t.
+     (\t. SND h' / (SND  h'+ FST h')) t +
+     (\t. FST h' / (SND h' + FST h') * exp (-(SND h' + FST h') * &t))t)--> (SND h' / (SND h' + FST h') + 0))` by RW_TAC real_ss[])
    ++ POP_ORW
    ++ MATCH_MP_TAC SEQ_ADD
    ++ RW_TAC std_ss[]
    >> (RW_TAC std_ss[SEQ_CONST])
-   >> ((`((\t. FST  h'/ (SND h' + FST h') * exp (-(SND h'  + FST h') * &t)) --> 0) = 
-      	  ((\t. (\t. FST h' / (SND h' + FST h')) t * 
-	  	(\t. exp (-(SND h' + FST h') * &t))t) --> 
-		((FST h' / (SND h' + FST h')) *0))` by RW_TAC real_ss[])
+   >> ((`((\t. FST  h'/ (SND h' + FST h') * exp (-(SND h'  + FST h') * &t)) --> 0) = ((\t. (\t. FST h' / (SND h' + FST h'))t * (\t. exp (-(SND h' + FST h') * &t))t) --> ((FST h' / (SND h' + FST h')) *0))` by RW_TAC real_ss[])
       ++ POP_ORW
       ++ MATCH_MP_TAC SEQ_MUL
       ++ RW_TAC real_ss[SEQ_CONST]
@@ -561,7 +564,7 @@ GEN_TAC
 ++ FIRST_X_ASSUM (Q.SPECL_THEN [`M`] MP_TAC)
 ++ RW_TAC std_ss[inst_avail_exp_list1_def, GSYM union_avail_event_list1_def]
 ++ FULL_SIMP_TAC list_ss[ inst_avail_exp_list1_def]);
-(*----------series_rbd_avail--------------------*)
+(*------------------------------*)
 val series_rbd_avail = store_thm("series_rbd_avail",
   ``!p L M.  
        prob_space p /\
@@ -595,6 +598,133 @@ RW_TAC std_ss[]
 ++ MATCH_MP_TAC series_expec_tends_prod_avail
 ++ RW_TAC std_ss[]);
 
+(*-------------------------*)
+val lim_inst_parall_tend_steady = store_thm("lim_inst_parall_tend_steady",
+  ``!p L M. 
+  prob_space p /\
+  (!z. MEM z M ==> (0 < FST z /\ 0 < SND z)) /\
+  (LENGTH L = LENGTH M) /\
+  (inst_avail_exp_list1 p L M) ==>
+  	((\t. list_prod
+     	       (one_minus_list
+		(list_prob p (union_avail_event_list1 L (&t)))))-->
+        compl_steady_state_avail M)  ``,
+GEN_TAC
+++ Induct
+>> (RW_TAC list_ss[LENGTH_NIL_SYM]
+   ++ RW_TAC list_ss[union_avail_event_list1_def,list_prod_def,list_prob_def,compl_steady_state_avail_def]
+   ++ RW_TAC std_ss[one_minus_list_def,list_prod_def,SEQ_CONST])
+++ GEN_TAC
+++ Induct
+>> (RW_TAC list_ss[])
+++  RW_TAC list_ss[union_avail_event_list1_def,list_prod_def,list_prob_def,compl_steady_state_avail_def]
+   ++ RW_TAC std_ss[one_minus_list_def,list_prod_def]
+++ (` (\t.
+   (1 - prob p (union_avail_events1 h (&t))) *
+   list_prod
+     (one_minus_list
+        (list_prob p (MAP (\a. union_avail_events1 a (&t)) L)))) = (\t.
+   (\t. (1 − prob p (union_avail_events1 h (&t)))) t *
+   (\t. list_prod
+     (one_minus_list
+        (list_prob p (MAP (\a. union_avail_events1 a (&t)) L)))) t)` by RW_TAC real_ss[])
+++ POP_ORW
+++ MATCH_MP_TAC SEQ_MUL
+++ RW_TAC std_ss[]
+>> ( (`(\t. 1 − prob p (union_avail_events1 h (&t))) = (\t. (\t. 1)t − (\t. prob p (union_avail_events1 h (&t))) t)` by RW_TAC real_ss[])
+   ++ POP_ORW
+   ++ MATCH_MP_TAC SEQ_SUB
+   ++ RW_TAC std_ss[SEQ_CONST]
+   ++ FULL_SIMP_TAC list_ss[inst_avail_exp_list1_def,inst_avail_exp2_def]
+   ++ REWRITE_TAC[steady_state_avail_def]
+   ++ (`((\t.
+     SND (h':real#real) / (SND h' + FST h') +
+     FST h' / (SND h' + FST h') * exp (-(SND h' + FST h') * &t))--> (SND h' / (SND h' + FST h'))) = ((\t.
+     (\t. SND h' / (SND  h'+ FST h')) t +
+     (\t. FST h' / (SND h' + FST h') * exp (-(SND h' + FST h') * &t))t)--> (SND h' / (SND h' + FST h') + 0))` by RW_TAC real_ss[])
+   ++ POP_ORW
+   ++ MATCH_MP_TAC SEQ_ADD
+   ++ RW_TAC std_ss[]
+   >> (RW_TAC std_ss[SEQ_CONST])
+   >> ((`((\t. FST  h'/ (SND h' + FST h') * exp (-(SND h'  + FST h') * &t)) --> 0) = ((\t. (\t. FST h' / (SND h' + FST h'))t * (\t. exp (-(SND h' + FST h') * &t))t) --> ((FST h' / (SND h' + FST h')) *0))` by RW_TAC real_ss[])
+      ++ POP_ORW
+      ++ MATCH_MP_TAC SEQ_MUL
+      ++ RW_TAC real_ss[SEQ_CONST]
+      ++ ONCE_REWRITE_TAC[REAL_MUL_SYM]
+      ++ RW_TAC std_ss[GSYM REAL_MUL_RNEG]
+      ++ MATCH_MP_TAC neg_exp_tend0_new
+      ++ RW_TAC std_ss[]
+      ++ RW_TAC std_ss[steady_avail_temp]))
+++ FIRST_X_ASSUM (Q.SPECL_THEN [`M`] MP_TAC)
+++ RW_TAC std_ss[inst_avail_exp_list1_def, GSYM union_avail_event_list1_def]
+++ FULL_SIMP_TAC list_ss[ inst_avail_exp_list1_def]);
+
+(*---compl_steady_state_avail_equi---------------------------*)
+val compl_steady_state_avail_equi = store_thm("compl_steady_state_avail_equi",
+  ``!M. compl_steady_state_avail M =  list_prod (one_minus_list (steady_state_avail_list M)) ``,
+Induct
+>> (RW_TAC list_ss[compl_steady_state_avail_def,steady_state_avail_list_def,one_minus_list_def,list_prod_def])
+++ RW_TAC list_ss[compl_steady_state_avail_def,steady_state_avail_list_def,one_minus_list_def,list_prod_def]);
+(*---parallel_steady_state_avail---------------------------*)
+val parallel_rbd_avail = store_thm("parallel_rbd_avail",
+  ``!p L M.  
+       prob_space p /\
+       (!z. MEM z M ==> 0 < FST z /\ 0 < SND z) /\
+       (LENGTH L = LENGTH M) /\
+       (!t'. ~NULL (union_avail_event_list1 L &t') /\
+       (!z. MEM z (union_avail_event_list1 L ( (&t'))) ==> z IN events p) /\
+       mutual_indep p (union_avail_event_list1 L ( (&t')))) /\
+       inst_avail_exp_list1 p L M ==> 
+        (lim (\t.  prob p 
+	     (rbd_struct p 
+	     	(parallel (rbd_list (union_avail_event_list1 L (&t)))))) =
+	  1 -  list_prod (one_minus_list (steady_state_avail_list M)))``,
+RW_TAC std_ss[]
+++ (`!t.  (prob p (rbd_struct p (parallel (rbd_list (union_avail_event_list1 L (&t))))) =
+      1 − list_prod (one_minus_list (list_prob p (union_avail_event_list1 L (&t)))))` by RW_TAC std_ss[])
+>> (MATCH_MP_TAC parallel_struct_thm
+   ++ FULL_SIMP_TAC std_ss[]
+   ++ RW_TAC std_ss[]
+   ++ FIRST_X_ASSUM(MP_TAC o Q.SPEC `t:num`)
+   ++ RW_TAC real_ss[])
+++ POP_ORW
+++ MATCH_MP_TAC SEQ_UNIQ
+++ EXISTS_TAC(--`(\t. 1 −
+       list_prod
+         (one_minus_list
+            (list_prob p (union_avail_event_list1 L (&t)))))`--)  
+++ RW_TAC std_ss[GSYM SEQ_LIM,convergent]
+>> (EXISTS_TAC(--` 1 -  list_prod (one_minus_list (steady_state_avail_list M))`--)
+   ++ (`(\t.
+        1 −
+        list_prod
+          (one_minus_list
+             (list_prob p (union_avail_event_list1 L (&t))))) = (\t.
+        (\t. 1) t −
+        (\t. list_prod
+          (one_minus_list
+             (list_prob p (union_avail_event_list1 L (&t))))) t)` by RW_TAC real_ss[])
+    ++ POP_ORW
+    ++ MATCH_MP_TAC SEQ_SUB
+    ++ RW_TAC std_ss[SEQ_CONST]
+    ++ RW_TAC std_ss[GSYM compl_steady_state_avail_equi]
+    ++ MATCH_MP_TAC lim_inst_parall_tend_steady
+    ++ RW_TAC std_ss[])
+++ (`(\t.
+        1 −
+        list_prod
+          (one_minus_list
+             (list_prob p (union_avail_event_list1 L (&t))))) = (\t.
+        (\t. 1) t −
+        (\t. list_prod
+          (one_minus_list
+             (list_prob p (union_avail_event_list1 L (&t))))) t)` by RW_TAC real_ss[])
+++ POP_ORW
+++ MATCH_MP_TAC SEQ_SUB
+++ RW_TAC std_ss[SEQ_CONST]
+++ RW_TAC std_ss[GSYM compl_steady_state_avail_equi]
+++ MATCH_MP_TAC lim_inst_parall_tend_steady
+++ RW_TAC std_ss[]);
 (*--------lim_inst_parall_series_tend_steady-----------------------------*)
 val lim_inst_parall_series_tend_steady = store_thm(
   "lim_inst_parall_series_tend_steady",
@@ -613,8 +743,7 @@ GEN_TAC
 ++ REWRITE_TAC[of_DEF,o_THM]
 ++ Induct
 >> (RW_TAC list_ss[LENGTH_NIL_SYM]
-   ++ RW_TAC list_ss[list_union_avail_event_list_def,steady_state_avail_prod_def,
-		     one_minus_list_def,list_prod_def]
+   ++ RW_TAC list_ss[list_union_avail_event_list_def,steady_state_avail_prod_def,one_minus_list_def,list_prod_def]
    ++ RW_TAC std_ss[SEQ_CONST])
 ++ GEN_TAC
 ++ Induct
@@ -637,9 +766,7 @@ GEN_TAC
 ++ POP_ORW
 ++ MATCH_MP_TAC SEQ_MUL
 ++ RW_TAC std_ss[]
->> ((`(\t. 1 − list_prod (list_prob p (union_avail_event_list1 h (&t)))) = 
-      (\t. (\t. 1) t − 
-      	   (\t. list_prod (list_prob p (union_avail_event_list1 h (&t)))) t)` by RW_TAC real_ss[])
+>> ((`(\t. 1 − list_prod (list_prob p (union_avail_event_list1 h (&t)))) = (\t. (\t. 1)t − (\t. list_prod (list_prob p (union_avail_event_list1 h (&t)))) t)` by RW_TAC real_ss[])
    ++ POP_ORW
    ++ MATCH_MP_TAC SEQ_SUB
    ++ RW_TAC std_ss[SEQ_CONST]
@@ -741,78 +868,7 @@ RW_TAC std_ss[]
   ++ MATCH_MP_TAC lim_inst_parall_series_tend_steady
   ++ METIS_TAC[]);
 
-(*-----------------------------------*)
-val compl_steady_state_avail_def = Define 
-`(compl_steady_state_avail [] = 1) /\
- (compl_steady_state_avail (h::t) = 
- (1 - steady_state_avail h) * compl_steady_state_avail (t))`;
-(*-------------------------*)
-val lim_inst_parall_tend_steady = store_thm("lim_inst_parall_tend_steady",
-  ``!p L M. 
-  prob_space p /\
-  (!z. MEM z M ==> (0 < FST z /\ 0 < SND z)) /\
-  (LENGTH L = LENGTH M) /\
-  (inst_avail_exp_list1 p L M) ==>
-  	((\t. list_prod
-     	       (one_minus_list
-		(list_prob p (union_avail_event_list1 L (&t)))))-->
-        compl_steady_state_avail M)  ``,
-GEN_TAC
-++ Induct
->> (RW_TAC list_ss[LENGTH_NIL_SYM]
-   ++ RW_TAC list_ss[union_avail_event_list1_def,list_prod_def,list_prob_def,compl_steady_state_avail_def]
-   ++ RW_TAC std_ss[one_minus_list_def,list_prod_def,SEQ_CONST])
-++ GEN_TAC
-++ Induct
->> (RW_TAC list_ss[])
-++  RW_TAC list_ss[union_avail_event_list1_def,list_prod_def,list_prob_def,compl_steady_state_avail_def]
-   ++ RW_TAC std_ss[one_minus_list_def,list_prod_def]
-++ (` (\t.
-   (1 - prob p (union_avail_events1 h (&t))) *
-   list_prod
-     (one_minus_list
-        (list_prob p (MAP (\a. union_avail_events1 a (&t)) L)))) = (\t.
-   (\t. (1 − prob p (union_avail_events1 h (&t)))) t *
-   (\t. list_prod
-     (one_minus_list
-        (list_prob p (MAP (\a. union_avail_events1 a (&t)) L)))) t)` by RW_TAC real_ss[])
-++ POP_ORW
-++ MATCH_MP_TAC SEQ_MUL
-++ RW_TAC std_ss[]
->> ( (`(\t. 1 − prob p (union_avail_events1 h (&t))) = 
-       (\t. (\t. 1)t − (\t. prob p (union_avail_events1 h (&t))) t)` by RW_TAC real_ss[])
-   ++ POP_ORW
-   ++ MATCH_MP_TAC SEQ_SUB
-   ++ RW_TAC std_ss[SEQ_CONST]
-   ++ FULL_SIMP_TAC list_ss[inst_avail_exp_list1_def,inst_avail_exp2_def]
-   ++ REWRITE_TAC[steady_state_avail_def]
-   ++ (`((\t.
-	  SND (h':real#real) / (SND h' + FST h') +
-     	  FST h' / (SND h' + FST h') * exp (-(SND h' + FST h') * &t)) --> 
-     	  (SND h' / (SND h' + FST h'))) = 
-	((\t.
-	   (\t. SND h' / (SND  h'+ FST h')) t +
-     	   (\t. FST h' / (SND h' + FST h') * exp (-(SND h' + FST h') * &t))t) --> 
-	   (SND h' / (SND h' + FST h') + 0))` by RW_TAC real_ss[])
-   ++ POP_ORW
-   ++ MATCH_MP_TAC SEQ_ADD
-   ++ RW_TAC std_ss[]
-   >> (RW_TAC std_ss[SEQ_CONST])
-   >> ((`((\t. FST  h'/ (SND h' + FST h') * exp (-(SND h'  + FST h') * &t)) --> 0) = 
-      	 ((\t. (\t. FST h' / (SND h' + FST h'))t * 
-	       (\t. exp (-(SND h' + FST h') * &t))t) --> 
-	        ((FST h' / (SND h' + FST h')) *0))` by RW_TAC real_ss[])
-      ++ POP_ORW
-      ++ MATCH_MP_TAC SEQ_MUL
-      ++ RW_TAC real_ss[SEQ_CONST]
-      ++ ONCE_REWRITE_TAC[REAL_MUL_SYM]
-      ++ RW_TAC std_ss[GSYM REAL_MUL_RNEG]
-      ++ MATCH_MP_TAC neg_exp_tend0_new
-      ++ RW_TAC std_ss[]
-      ++ RW_TAC std_ss[steady_avail_temp]))
-++ FIRST_X_ASSUM (Q.SPECL_THEN [`M`] MP_TAC)
-++ RW_TAC std_ss[inst_avail_exp_list1_def, GSYM union_avail_event_list1_def]
-++ FULL_SIMP_TAC list_ss[ inst_avail_exp_list1_def]);
+
 
 (*------------------------*)
 val lim_inst_series_parall_tend_steady = store_thm(
@@ -922,101 +978,89 @@ RW_TAC std_ss[]
 ++ RW_TAC std_ss[]);
 
 (*--------------------------------------------------------*)
-(* Definition. Unavailability Event			  *)
-(* -------------------------------------------------------*)
+(* Definition. Unavailability Event       *)
+(* ------------------------------------------------------------------------- *)
 val unavail_event_def =  Define `unavail_event p L n t  =  
 p_space p DIFF (avail_event L n t INTER p_space p)`;
 (*--------------------------------------------------------*)
-(* Definition. Union Unavailability Event		  *)
-(* -------------------------------------------------------*)
-val union_unavail_events_def =  Define 
-`union_unavail_events p L t  =  
+(* Definition. Union Unavailability Event       *)
+(* ------------------------------------------------------------------------- *)
+val union_unavail_events_def =  Define `union_unavail_events p L t  =  
 p_space p DIFF (union_avail_events1 L t INTER p_space p)`;
-(*--------------------------------------------------------*)
-(* Definition : Unavailability event list                 *)
-(* ------------------------------------------------------ *)
+(*---------------------------------------------------------*)
+(* Definition : Unavailability event list                   *)
+(* ------------------------------------------------------------------------- *)
 val union_unavail_event_list_def = Define 
 `union_unavail_event_list p L t  =  
 MAP (\a. union_unavail_events p a t) L`;
-(*--------------------------------------------------------*)
-(* Definition : list Unavailability event list            *)
-(* ------------------------------------------------------ *)
-val list_union_unavail_event_list_def = Define 
-`list_union_unavail_event_list p L t  =  
-MAP (\a. union_unavail_event_list p a t) L`;
-(* ------------------------------------------------------ *)
-(* Definition: steady state unavailiabilility 
-   	       with failure and repair rate               *)
-(* ------------------------------------------------------ *)
+(* ------------------------------------------------------------------------- *)
+(* Definition: steady state unavailiabilility with failure and repair rate                               *)
+(* ------------------------------------------------------------------------- *)
 val steady_state_unavail_def = Define 
-`(steady_state_unavail (m:real#real) = 
-  FST m / (SND m + FST m))`;
-(* ------------------------------------------------------ *)
-(* Definition: steady state unavailiabilility 
-   	       with failure and repair rate  list         *)
-(* ------------------------------------------------------ *)
+`( steady_state_unavail (m:real#real) = FST m / (SND m + FST m))`;
+
+(* ------------------------------------------------------------------------- *)
+(* Definition: steady state unavailiabilility with failure and repair rate  list                             *)
+(* ------------------------------------------------------------------------- *)
 val steady_state_unavail_list_def = Define 
-`(steady_state_unavail_list M = 
-  MAP (\a. steady_state_unavail a) M) `;
+`( steady_state_unavail_list M = MAP (\a. steady_state_unavail a) M) `;
 
 (*---------------------------------------------------------*)
-(* Definition: Instantenous Unavailability pair            *)
-(* ------------------------------------------------------- *)
+(* Definition: Instantenous Unavailability pair                  *)
+(* ------------------------------------------------------------------------- *)
+(*-------------------------*)
 val inst_unavail_exp_def = Define 
 `inst_unavail_exp p L m = 
  !(t). (prob p ( union_unavail_events p L &t)  =  
        (FST (m) / (SND m + FST m)) - 
        (FST m /(SND m + FST m)) * exp (-((SND m + FST m))* &t)) `;
 (*-------------------------*)
-val inst_unavail_exp_list_def = Define 
-`(inst_unavail_exp_list p [] M = T) /\ 
- (inst_unavail_exp_list p (h::t) M = 
-  inst_unavail_exp p h (HD M) /\ inst_unavail_exp_list p t (TL M) ) `;
-(*---------------------------------------------------------*)
+val inst_unavail_exp_list_def = Define `(inst_unavail_exp_list p [] M = T) /\ (inst_unavail_exp_list p (h::t) M = inst_unavail_exp p h (HD M) /\ inst_unavail_exp_list p t (TL M) ) `;
+(*-------------------------*)
 val two_dim_inst_unavail_exp_def = Define 
 `(two_dim_inst_unavail_exp p [] M = T) /\ 
  (two_dim_inst_unavail_exp p (h::t) M = 
-  inst_unavail_exp_list p h (HD M) /\ 
-  two_dim_inst_unavail_exp p t (TL M)) `;
-(* -------------------------------------------------------- *)
-(*--- Definition.  Unavailability FT gates     		    *)
-(* -------------------------------------------------------- *)
-(* -------------------------------------------------------- *)
-(*--- Definition. AND unavail FT gate     		    *)
-(* -------------------------------------------------------- *)
+  inst_unavail_exp_list p h (HD M) /\ two_dim_inst_unavail_exp p t (TL M) ) `;
+
+(* ------------------------------------------------------------------------- *)
+(*--- Definition.  Unavailability FT gates     ----  *)
+(* ------------------------------------------------------------------------- *)
+(* ------------------------------------------------------------------------- *)
+(*--- Definition. AND unavail FT gate     ----  *)
+(* ------------------------------------------------------------------------- *)
 val AND_unavail_FT_gate_def =  Define
 `!L p. AND_unavail_FT_gate p L t = 
        FTree p (AND (gate_list (union_unavail_event_list p L t)))`;
-(* -------------------------------------------------------- *)
-(* Definition. OR unavail FT gate                           *)
-(* -------------------------------------------------------- *)
+(* ------------------------------------------------------------------------- *)
+(* Definition. OR unavail FT gate                                 *)
+(* ------------------------------------------------------------------------- *)
 val OR_unavail_FT_gate_def =  Define
 `!L p. OR_unavail_FT_gate p L t = 
        FTree p (OR (gate_list (union_unavail_event_list p L t)))`;
-(* -------------------------------------------------------- *)
-(* Definition. NOR unavail FT gate                          *)
-(* -------------------------------------------------------- *)
+(* ------------------------------------------------------------------------- *)
+(* Definition. NOR unavail FT gate                                 *)
+(* ------------------------------------------------------------------------- *)
 val NOR_unavail_FT_gate_def =  Define
 `!L p. NOR_unavail_FT_gate p L t  =
        p_space p DIFF FTree p (OR (gate_list (union_unavail_event_list p L t)))`;
-(* -------------------------------------------------------- *)
-(* Definition. NAND unavail FT gate                         *)
-(* -------------------------------------------------------- *)
+(* ------------------------------------------------------------------------- *)
+(* Definition. NAND unavail FT gate                                 *)
+(* ------------------------------------------------------------------------- *)
 val NAND_unavail_FT_gate_def =  Define
 `!L1 L2 p t. NAND_unavail_FT_gate p L1 L2 t  =
      	     FTree p 
 	       (AND (gate_list (compl_list p (union_unavail_event_list p L1 t) ++
 	     	     	  	             (union_unavail_event_list p L2 t))))`;
 
-(* -------------------------------------------------------- *)
-(* Definition. XOR unavail FT gate                          *)
-(* -------------------------------------------------------- *)
+(* ------------------------------------------------------------------------- *)
+(* Definition. XOR unavail FT gate                                 *)
+(* ------------------------------------------------------------------------- *)
 val XOR_unavail_FT_gate_def =  Define
 `!p X Y t. XOR_unavail_FT_gate p X Y t  =
       	   (XOR_FT_gate p (atomic (union_unavail_events p X t)) 
 	   		  (atomic (union_unavail_events p Y t)))`;
 
-(*----------------------------------------------------------*)
+(*---------------------------------------*)
 val AND_inst_avail_prod_tends_steady = store_thm(
   "AND_inst_avail_prod_tends_steady",
   `` !p L M.
@@ -1027,14 +1071,12 @@ val AND_inst_avail_prod_tends_steady = store_thm(
 GEN_TAC
 ++ Induct
 >> (RW_TAC list_ss[LENGTH_NIL_SYM]
-   ++ RW_TAC list_ss[union_unavail_event_list_def,list_prod_def,
-		     list_prob_def,steady_state_unavail_list_def]
+   ++ RW_TAC list_ss[union_unavail_event_list_def,list_prod_def,list_prob_def,steady_state_unavail_list_def]
    ++ RW_TAC std_ss[SEQ_CONST])
 ++ GEN_TAC
 ++ Induct
 >> (RW_TAC list_ss[])
-++  RW_TAC list_ss[union_unavail_event_list_def,list_prod_def,
-		   list_prob_def,steady_state_unavail_list_def] 
+++  RW_TAC list_ss[union_unavail_event_list_def,list_prod_def,list_prob_def,steady_state_unavail_list_def] 
 ++ (`!t. (
    prob p (union_unavail_events p h (&t)) *
    list_prod
@@ -1051,18 +1093,14 @@ GEN_TAC
    ++ REWRITE_TAC[steady_state_unavail_def]
    ++ (`((\t.
      FST (h':real#real) / (SND h' + FST h') -
-     FST h' / (SND h' + FST h') * exp (-(SND h' + FST h') * &t))--> (FST h' / (SND h' + FST h'))) = 
-     ((\t.
+     FST h' / (SND h' + FST h') * exp (-(SND h' + FST h') * &t))--> (FST h' / (SND h' + FST h'))) = ((\t.
      (\t. FST (h':real#real) / (SND  h'+ FST h')) t -
-     (\t. FST h' / (SND h' + FST h') * exp (-(SND h' + FST h') * &t))t) --> 
-     (FST h' / (SND h' + FST h') - 0))` by RW_TAC real_ss[])
+     (\t. FST h' / (SND h' + FST h') * exp (-(SND h' + FST h') * &t))t)--> (FST h' / (SND h' + FST h') - 0))` by RW_TAC real_ss[])
    ++ POP_ORW
    ++ MATCH_MP_TAC SEQ_SUB
    ++ RW_TAC std_ss[]
    >> (RW_TAC std_ss[SEQ_CONST])
-   >> ((`((\t. FST  h'/ (SND h' + FST h') * exp (-(SND h'  + FST h') * &t)) --> 0) = 
-      ((\t. (\t. FST h' / (SND h' + FST h'))t * (\t. exp (-(SND h' + FST h') * &t))t) --> 
-      	    ((FST h' / (SND h' + FST h')) *0))` by RW_TAC real_ss[])
+   >> ((`((\t. FST  h'/ (SND h' + FST h') * exp (-(SND h'  + FST h') * &t)) --> 0) = ((\t. (\t. FST h' / (SND h' + FST h'))t * (\t. exp (-(SND h' + FST h') * &t))t) --> ((FST h' / (SND h' + FST h')) *0))` by RW_TAC real_ss[])
       ++ POP_ORW
       ++ MATCH_MP_TAC SEQ_MUL
       ++ RW_TAC real_ss[SEQ_CONST]
@@ -1072,9 +1110,8 @@ GEN_TAC
       ++ RW_TAC std_ss[]
       ++ RW_TAC std_ss[steady_avail_temp]))
 ++ FIRST_X_ASSUM (Q.SPECL_THEN [`M`] MP_TAC)
-++ FULL_SIMP_TAC std_ss[inst_unavail_exp_list_def,GSYM union_unavail_event_list_def,
-   		 	GSYM steady_state_unavail_list_def]
-++ FULL_SIMP_TAC list_ss[inst_unavail_exp_list_def]);
+++ FULL_SIMP_TAC std_ss[inst_unavail_exp_list_def, GSYM union_unavail_event_list_def, GSYM steady_state_unavail_list_def]
+++ FULL_SIMP_TAC list_ss[ inst_unavail_exp_list_def]);
 
 (*---------------------------*)
 val AND_gate_unavail = store_thm("AND_gate_unavail",
@@ -1108,7 +1145,7 @@ RW_TAC std_ss[]
 ++ MATCH_MP_TAC AND_inst_avail_prod_tends_steady
 ++ RW_TAC std_ss[]);
    
-(*-------------------------------------------------------------*)
+(*-------------------*)
 val lim_inst_OR_tend_steady = store_thm("lim_inst_OR_tend_steady",
   ``!p L M. prob_space p /\
        	    (!z. MEM z M ==> (0 < FST z /\ 0 < SND z)) /\
@@ -1122,14 +1159,12 @@ val lim_inst_OR_tend_steady = store_thm("lim_inst_OR_tend_steady",
 GEN_TAC
 ++ Induct
 >> (RW_TAC list_ss[LENGTH_NIL_SYM]
-   ++ RW_TAC list_ss[union_unavail_event_list_def,list_prod_def,
-		     list_prob_def,steady_state_unavail_list_def]
+   ++ RW_TAC list_ss[union_unavail_event_list_def,list_prod_def,list_prob_def,steady_state_unavail_list_def]
    ++ RW_TAC std_ss[one_minus_list_def,list_prod_def,SEQ_CONST])
 ++ GEN_TAC
 ++ Induct
 >> (RW_TAC list_ss[])
-++  RW_TAC list_ss[union_unavail_event_list_def,list_prod_def,
-		   list_prob_def,steady_state_unavail_list_def]
+++  RW_TAC list_ss[union_unavail_event_list_def,list_prod_def,list_prob_def,steady_state_unavail_list_def]
    ++ RW_TAC std_ss[one_minus_list_def,list_prod_def]
 ++ (` (\t.
    (1 - prob p (union_unavail_events p h (&t))) *
@@ -1143,8 +1178,7 @@ GEN_TAC
 ++ POP_ORW
 ++ MATCH_MP_TAC SEQ_MUL
 ++ RW_TAC std_ss[]
->> ( (`(\t. 1 − prob p (union_unavail_events p h (&t))) = 
-       (\t. (\t. 1)t − (\t. prob p (union_unavail_events p h (&t))) t)` by RW_TAC real_ss[])
+>> ( (`(\t. 1 − prob p (union_unavail_events p h (&t))) = (\t. (\t. 1)t − (\t. prob p (union_unavail_events p h (&t))) t)` by RW_TAC real_ss[])
    ++ POP_ORW
    ++ MATCH_MP_TAC SEQ_SUB
    ++ RW_TAC std_ss[SEQ_CONST]
@@ -1159,9 +1193,7 @@ GEN_TAC
    ++ MATCH_MP_TAC SEQ_SUB
    ++ RW_TAC std_ss[]
    >> (RW_TAC std_ss[SEQ_CONST])
-   >> ((`((\t. FST  h'/ (SND h' + FST h') * exp (-(SND h'  + FST h') * &t)) --> 0) = 
-      	 ((\t. (\t. FST h' / (SND h' + FST h'))t * (\t. exp (-(SND h' + FST h') * &t))t) --> 
-	       ((FST h' / (SND h' + FST h')) *0))` by RW_TAC real_ss[])
+   >> ((`((\t. FST  h'/ (SND h' + FST h') * exp (-(SND h'  + FST h') * &t)) --> 0) = ((\t. (\t. FST h' / (SND h' + FST h'))t * (\t. exp (-(SND h' + FST h') * &t))t) --> ((FST h' / (SND h' + FST h')) *0))` by RW_TAC real_ss[])
       ++ POP_ORW
       ++ MATCH_MP_TAC SEQ_MUL
       ++ RW_TAC real_ss[SEQ_CONST]
@@ -1171,8 +1203,7 @@ GEN_TAC
       ++ RW_TAC std_ss[]
       ++ RW_TAC std_ss[steady_avail_temp]))
 ++ FIRST_X_ASSUM (Q.SPECL_THEN [`M`] MP_TAC)
-++ RW_TAC std_ss[inst_unavail_exp_list_def, GSYM union_unavail_event_list_def,
-   	  	 GSYM steady_state_unavail_list_def]
+++ RW_TAC std_ss[inst_unavail_exp_list_def, GSYM union_unavail_event_list_def,GSYM steady_state_unavail_list_def]
 ++ FULL_SIMP_TAC list_ss[ inst_unavail_exp_list_def]);
 
 (*----------------------------*)
@@ -1194,8 +1225,7 @@ RW_TAC std_ss[]
 ++ (`!t.  
       prob p
        (FTree p (OR (gate_list (union_unavail_event_list p L (&t))))) =
-      1 - list_prod (one_minus_list 
-      	  	    (list_prob p (union_unavail_event_list p L (&t))))` by RW_TAC std_ss[])
+      1 - list_prod (one_minus_list (list_prob p (union_unavail_event_list p L (&t))))` by RW_TAC std_ss[])
 >> (MATCH_MP_TAC OR_gate_thm 
    ++ METIS_TAC[])
 ++ POP_ORW
@@ -1257,8 +1287,7 @@ RW_TAC std_ss[NOR_unavail_FT_gate_def]
 ++ POP_ORW
 ++ (`!t.  prob p
        (FTree p (OR (gate_list (union_unavail_event_list p L (&t))))) =
-        1 - list_prod 
-	  (one_minus_list (list_prob p (union_unavail_event_list p L (&t))))` by RW_TAC std_ss[])
+        1 - list_prod (one_minus_list (list_prob p (union_unavail_event_list p L (&t))))` by RW_TAC std_ss[])
 >> (MATCH_MP_TAC OR_gate_thm
    ++ METIS_TAC[])
 ++ POP_ORW
@@ -1273,12 +1302,9 @@ RW_TAC std_ss[NOR_unavail_FT_gate_def]
    ++ RW_TAC std_ss[])
 ++ MATCH_MP_TAC lim_inst_OR_tend_steady
 ++ RW_TAC std_ss[]);
-(*----------------------------------------------------------------------*)
+(*------------------------*)
 val in_events_normal_events = store_thm("in_events_normal_events",
-  ``!p A t. 
-       prob_space p /\ 
-       (p_space p DIFF (A INTER p_space p) IN events p) ==> 
-       	 (A INTER p_space p IN events p)  ``,
+  ``!p A t. prob_space p /\ (p_space p DIFF (A INTER p_space p) IN events p) ==> (A INTER p_space p IN events p)  ``,
  REPEAT GEN_TAC
  ++ RW_TAC std_ss[]
  ++ (`A INTER p_space p = p_space p DIFF (p_space p DIFF (A INTER p_space p))` by MATCH_MP_TAC EQ_SYM)
@@ -1287,8 +1313,10 @@ val in_events_normal_events = store_thm("in_events_normal_events",
  ++ POP_ORW
  ++ MATCH_MP_TAC EVENTS_COMPL
  ++ RW_TAC std_ss[]);
-(*----------------------------------------------------------------------*)
-val lim_inst_NAND_tend_steady = store_thm("lim_inst_NAND_tend_steady",
+
+
+(*-------------------------*)
+val lim_inst_NAND_tend_steady = store_thm("lim_inst_OR_tend_steady",
   ``!p L M. prob_space p /\
        	    (!z. MEM z M ==> (0 < FST z /\ 0 < SND z)) /\
  	    (LENGTH L = LENGTH M) /\ 
@@ -1303,14 +1331,12 @@ val lim_inst_NAND_tend_steady = store_thm("lim_inst_NAND_tend_steady",
 GEN_TAC
 ++ Induct
 >> (RW_TAC list_ss[LENGTH_NIL_SYM]
-   ++ RW_TAC list_ss[union_unavail_event_list_def,list_prod_def,
-		     list_prob_def,steady_state_avail_list_def,compl_list_def]
+   ++ RW_TAC list_ss[union_unavail_event_list_def,list_prod_def,list_prob_def,steady_state_avail_list_def,compl_list_def]
    ++ RW_TAC std_ss[SEQ_CONST])
 ++ GEN_TAC
 ++ Induct
 >> (RW_TAC list_ss[])
-++  RW_TAC list_ss[union_unavail_event_list_def,list_prod_def,list_prob_def,
-		   steady_state_avail_list_def,compl_list_def]
+++  RW_TAC list_ss[union_unavail_event_list_def,list_prod_def,list_prob_def,steady_state_avail_list_def,compl_list_def]
    ++ RW_TAC std_ss[one_minus_list_def,list_prod_def]
 ++ (` (\t.
    prob p (p_space p DIFF union_unavail_events p h (&t)) *
@@ -1328,8 +1354,7 @@ GEN_TAC
 ++ RW_TAC std_ss[]
 >> ( RW_TAC std_ss[union_unavail_events_def]
    ++ (`!t. (p_space p DIFF
-      	     	 (p_space p DIFF union_avail_events1 h (&t) INTER p_space p)) = 
-      	     union_avail_events1 h (&t) INTER p_space p ` by RW_TAC std_ss[])
+      (p_space p DIFF union_avail_events1 h (&t) INTER p_space p)) = union_avail_events1 h (&t) INTER p_space p ` by RW_TAC std_ss[])
       >> ( DEP_REWRITE_TAC[DIFF_DIFF_SUBSET]
       	 ++ RW_TAC std_ss[INTER_SUBSET])
       ++ POP_ORW
@@ -1337,18 +1362,14 @@ GEN_TAC
       ++ RW_TAC std_ss[steady_state_avail_def]
       ++ (`((\t.
      SND (h':real#real) / (SND h' + FST h') +
-     FST h' / (SND h' + FST h') * exp (-(SND h' + FST h') * &t))--> (SND h' / (SND h' + FST h'))) = 
-     	 ((\t.
-     	  (\t. SND h' / (SND  h'+ FST h')) t +
-     	  (\t. FST h' / (SND h' + FST h') * exp (-(SND h' + FST h') * &t))t) --> 
-	  (SND h' / (SND h' + FST h') + 0))` by RW_TAC real_ss[])
+     FST h' / (SND h' + FST h') * exp (-(SND h' + FST h') * &t))--> (SND h' / (SND h' + FST h'))) = ((\t.
+     (\t. SND h' / (SND  h'+ FST h')) t +
+     (\t. FST h' / (SND h' + FST h') * exp (-(SND h' + FST h') * &t))t)--> (SND h' / (SND h' + FST h') + 0))` by RW_TAC real_ss[])
    ++ POP_ORW
    ++ MATCH_MP_TAC SEQ_ADD
    ++ RW_TAC std_ss[]
    >> (RW_TAC std_ss[SEQ_CONST])
-   >> ((`((\t. FST  h'/ (SND h' + FST h') * exp (-(SND h'  + FST h') * &t)) --> 0) = 
-      	  ((\t. (\t. FST h' / (SND h' + FST h'))t * (\t. exp (-(SND h' + FST h') * &t))t) --> 
-	  	((FST h' / (SND h' + FST h')) *0))` by RW_TAC real_ss[])
+   >> ((`((\t. FST  h'/ (SND h' + FST h') * exp (-(SND h'  + FST h') * &t)) --> 0) = ((\t. (\t. FST h' / (SND h' + FST h'))t * (\t. exp (-(SND h' + FST h') * &t))t) --> ((FST h' / (SND h' + FST h')) *0))` by RW_TAC real_ss[])
       ++ POP_ORW
       ++ MATCH_MP_TAC SEQ_MUL
       ++ RW_TAC real_ss[SEQ_CONST]
@@ -1366,6 +1387,8 @@ GEN_TAC
    >> (FIRST_X_ASSUM (Q.SPECL_THEN [`t'`,`z`] MP_TAC)
       ++ RW_TAC list_ss[])
    ++ METIS_TAC[GSYM compl_list_def]);
+
+
 (*-------------------------*)
 val NAND_steady_state_avail = store_thm("NAND_steady_state_avail",
   ``!p L1 L2 M1 M2.
@@ -1400,7 +1423,7 @@ RW_TAC std_ss[]
             (compl_list p (union_unavail_event_list p L1 (&t)))) *
        list_prod (list_prob p (union_unavail_event_list p L2 (&t))))`--)  
 ++ RW_TAC std_ss[GSYM SEQ_LIM,convergent]
->> (EXISTS_TAC(--`( list_prod (steady_state_avail_list M1)*list_prod (steady_state_unavail_list M2))`--)
+>> (EXISTS_TAC(--`( list_prod (steady_state_avail_list M1) *list_prod (steady_state_unavail_list M2))`--)
    ++ (`(\t.
    list_prod
      (list_prob p (compl_list p (union_unavail_event_list p L1 (&t)))) *
@@ -1449,18 +1472,14 @@ RW_TAC std_ss[]
      ++ RW_TAC std_ss[steady_state_unavail_def]
      ++ (`((\t.
      FST (m1:real#real) / (SND m1 + FST m1) -
-     FST m1 / (SND m1 + FST m1) * exp (-(SND m1 + FST m1) * &t))--> (FST m1 / (SND m1 + FST m1))) = 
-     ((\t.
+     FST m1 / (SND m1 + FST m1) * exp (-(SND m1 + FST m1) * &t))--> (FST m1 / (SND m1 + FST m1))) = ((\t.
      (\t. FST m1 / (SND  m1+ FST m1)) t -
-     (\t. FST m1 / (SND m1 + FST m1) * exp (-(SND m1 + FST m1) * &t))t) --> 
-     	  (FST m1 / (SND m1 + FST m1) - 0))` by RW_TAC real_ss[])
+     (\t. FST m1 / (SND m1 + FST m1) * exp (-(SND m1 + FST m1) * &t))t)--> (FST m1 / (SND m1 + FST m1) - 0))` by RW_TAC real_ss[])
    ++ POP_ORW
    ++ MATCH_MP_TAC SEQ_SUB
    ++ RW_TAC std_ss[]
    >> (RW_TAC std_ss[SEQ_CONST])
-   ++ (`((\t. FST  (m1:real#real) / (SND m1 + FST m1) * exp (-(SND m1  + FST m1) * &t)) --> 0) = 
-      	 ((\t. (\t. FST m1 / (SND m1 + FST m1))t * (\t. exp (-(SND m1 + FST m1) * &t))t) --> 
-	       ((FST m1 / (SND m1 + FST m1)) *0))` by RW_TAC real_ss[])
+   ++ (`((\t. FST  (m1:real#real) / (SND m1 + FST m1) * exp (-(SND m1  + FST m1) * &t)) --> 0) = ((\t. (\t. FST m1 / (SND m1 + FST m1))t * (\t. exp (-(SND m1 + FST m1) * &t))t) --> ((FST m1 / (SND m1 + FST m1)) *0))` by RW_TAC real_ss[])
       ++ POP_ORW
       ++ MATCH_MP_TAC SEQ_MUL
       ++ RW_TAC real_ss[SEQ_CONST]
@@ -1492,12 +1511,8 @@ val XOR_steady_unavail = store_thm("XOR_steady_unavail",
        steady_state_unavail m2 * (1 - steady_state_unavail m1))``,
 RW_TAC std_ss[]
 ++ (`!t. prob p
-       	  (XOR_FT_gate p (atomic (union_unavail_events p X1 &t))
-       	     	       	 (atomic (union_unavail_events p X2 &t))) =  
-	prob p (union_unavail_events p X1 (&t)) * 
-	 (1 - prob p (union_unavail_events p X2 (&t))) + 
-	  prob p  (union_unavail_events p X2 (&t)) * 
-	  (1- prob p (union_unavail_events p X1 (&t)))` by RW_TAC std_ss[])
+       (XOR_FT_gate p (atomic (union_unavail_events p X1 &t))
+       	     	      (atomic (union_unavail_events p X2 &t))) =  prob p(union_unavail_events p X1 (&t))  * (1 - prob p (union_unavail_events p X2 (&t))) + prob p  (union_unavail_events p X2 (&t)) * (1- prob p (union_unavail_events p X1 (&t)))` by RW_TAC std_ss[])
 >> (MATCH_MP_TAC XOR_FT_gate_thm
    ++ METIS_TAC[])
 ++ POP_ORW
@@ -1533,8 +1548,7 @@ RW_TAC std_ss[]
      ++ RW_TAC std_ss[]
      >> ( MATCH_MP_TAC inst_XOR_tends_steady
      	++ METIS_TAC[])
-     ++ (`(\t. 1 − prob p (union_unavail_events p X2 (&t))) = 
-     	  (\t. (\t. 1) t − (\t. prob p (union_unavail_events p X2 (&t))) t)` by RW_TAC real_ss[])
+     ++ (`(\t. 1 − prob p (union_unavail_events p X2 (&t))) =(\t. (\t. 1) t − (\t. prob p (union_unavail_events p X2 (&t))) t) `  by RW_TAC real_ss[])
      ++ POP_ORW
      ++ MATCH_MP_TAC SEQ_SUB
      ++ RW_TAC std_ss[SEQ_CONST]
@@ -1550,8 +1564,7 @@ RW_TAC std_ss[]
   ++ RW_TAC std_ss[]
   >> (MATCH_MP_TAC inst_XOR_tends_steady
      ++ METIS_TAC[])
-  ++ (`(\t. 1 − prob p (union_unavail_events p X1 (&t))) = 
-       (\t. (\t. 1) t − (\t. prob p (union_unavail_events p X1 (&t))) t) `  by RW_TAC real_ss[])
+  ++ (`(\t. 1 − prob p (union_unavail_events p X1 (&t))) =(\t. (\t. 1) t − (\t. prob p (union_unavail_events p X1 (&t))) t) `  by RW_TAC real_ss[])
   ++ POP_ORW
   ++ MATCH_MP_TAC SEQ_SUB
   ++ RW_TAC std_ss[SEQ_CONST]
@@ -1561,7 +1574,7 @@ RW_TAC std_ss[]
    prob p (union_unavail_events p X1 (&t)) *
    (1 − prob p (union_unavail_events p X2 (&t))) +
    prob p (union_unavail_events p X2 (&t)) *
-   (1 − prob p (union_unavail_events p X1 (&t)))) = (\t.
+   (1 − prob p (union_unavail_events p X1 (&t)))) =(\t.
    (\t. prob p (union_unavail_events p X1 (&t)) *
    (1 − prob p (union_unavail_events p X2 (&t)))) t +
    (\t. prob p (union_unavail_events p X2 (&t)) *
@@ -1579,8 +1592,7 @@ RW_TAC std_ss[]
      ++ RW_TAC std_ss[]
      >> ( MATCH_MP_TAC inst_XOR_tends_steady
      	++ METIS_TAC[])
-     ++ (`(\t. 1 − prob p (union_unavail_events p X2 (&t))) = 
-     	  (\t. (\t. 1) t − (\t. prob p (union_unavail_events p X2 (&t))) t) ` by RW_TAC real_ss[])
+     ++ (`(\t. 1 − prob p (union_unavail_events p X2 (&t))) =(\t. (\t. 1) t − (\t. prob p (union_unavail_events p X2 (&t))) t) `  by RW_TAC real_ss[])
      ++ POP_ORW
      ++ MATCH_MP_TAC SEQ_SUB
      ++ RW_TAC std_ss[SEQ_CONST]
@@ -1596,895 +1608,10 @@ RW_TAC std_ss[]
   ++ RW_TAC std_ss[]
   >> (MATCH_MP_TAC inst_XOR_tends_steady
      ++ METIS_TAC[])
-  ++ (`(\t. 1 − prob p (union_unavail_events p X1 (&t))) = 
-       (\t. (\t. 1) t − (\t. prob p (union_unavail_events p X1 (&t))) t) ` by RW_TAC real_ss[])
+  ++ (`(\t. 1 − prob p (union_unavail_events p X1 (&t))) =(\t. (\t. 1) t − (\t. prob p (union_unavail_events p X1 (&t))) t) `  by RW_TAC real_ss[])
   ++ POP_ORW
   ++ MATCH_MP_TAC SEQ_SUB
   ++ RW_TAC std_ss[SEQ_CONST]
   ++ MATCH_MP_TAC inst_XOR_tends_steady
   ++ METIS_TAC[]);
-
-(*-----------Case Study Theorems-----------*)
-val solar_array_RBD_avail = store_thm("solar_array_RBD_avail",
-  ``!p R1 R2 R3 R4 R5 M1 M2 M3 M4 M5.  
-       prob_space p /\ 
-       (!z. MEM z (FLAT [[M1;M1];[M2];[M3;M3];[M4];[M4];[M5;M5]]) ==> 
-       	    0 < FST z /\ 0 < SND z) /\
-       (!t'. 
-        (!z. MEM z 
-	     (FLAT (list_union_avail_event_list 
-	     	   ([[R1;R1];[R2];[R3;R3];[R4];[R4];[R5;R5]]) (&t'))) ==> z IN events p) /\
-       mutual_indep p 
-	 (FLAT (list_union_avail_event_list 
-	       ([[R1;R1];[R2];[R3;R3];[R4];[R4];[R5;R5]]) (&t')))) /\ 
-       (two_dim_inst_avail_exp p 
-       		([[R1;R1];[R2];[R3;R3];[R4];[R4];[R5;R5]]) 
-		([[M1;M1];[M2];[M3;M3];[M4];[M4];[M5;M5]])) ==> 
-	  
-	  (lim (\t. prob p 
-	      (rbd_struct p
-                     ((series of (λa. parallel (rbd_list a)))
-                        (list_union_avail_event_list 
-				([[R1;R1];[R2];[R3;R3];[R4];[R4];[R5;R5]]) (&t))))) =
-       	  list_prod 
-	    (one_minus_list (MAP 
-	       (\a. compl_steady_state_avail a) 
-	       	    ([[M1;M1];[M2];[M3;M3];[M4];[M4];[M5;M5]]))))``,
-RW_TAC std_ss[]
-++ MATCH_MP_TAC steady_state_series_parallel_avail
-++ RW_TAC list_ss[]
->> (RW_TAC list_ss[]
-   ++ Cases_on `n`
-   >> (RW_TAC list_ss[])
-   ++ RW_TAC list_ss[]
-   ++ Cases_on `n'`
-   >> (RW_TAC list_ss[])
-   ++ RW_TAC list_ss[]
-   ++ Cases_on `n`
-   >> (RW_TAC list_ss[])
-  ++ RW_TAC list_ss[]
-   ++ Cases_on `n'`
-   >> (RW_TAC list_ss[])
-   ++ RW_TAC list_ss[]
-   ++ Cases_on `n`
-   >> (RW_TAC list_ss[])
-   ++ RW_TAC list_ss[]
-   ++ Cases_on `n'`
-   >> (RW_TAC list_ss[])
-   ++ RW_TAC list_ss[])
->> (RW_TAC list_ss[]
-   >> (FULL_SIMP_TAC list_ss[list_union_avail_event_list_def]
-      >> (RW_TAC list_ss[union_avail_event_list1_def])
-      >> (RW_TAC list_ss[union_avail_event_list1_def])
-      >> (RW_TAC list_ss[union_avail_event_list1_def])
-      >> (RW_TAC list_ss[union_avail_event_list1_def])
-      >> (RW_TAC list_ss[union_avail_event_list1_def])
-   ++ (RW_TAC list_ss[union_avail_event_list1_def]))
-   ++ FIRST_X_ASSUM (Q.SPECL_THEN [`t'`] MP_TAC)
-   ++ RW_TAC std_ss[])
-   ++ METIS_TAC[]);
-
-(*--------------------------------------------------*)
-
-val solar_array_FT_def = Define 
-`solar_array_FT p x1 x2 x3 x4 x5 x6 x7 x8 x9 x10 x11 x12 x13 x14 t =
- FTree p (OR [OR (gate_list (union_unavail_event_list p [x1;x2;x3;x4] t));
-       	      AND (gate_list (union_unavail_event_list p [x5;x6] t));
-	      OR (gate_list (union_unavail_event_list p [x7;x8;x9;x10;x11;x12;x13;x14] t))]) `;
-
-(*-------------------------------------------------*)
-
-val solar_array_FT_to_RBD = store_thm("solar_array_FT_to_RBD",
-  ``!p x1 x2 x3 x4 x5 x6 x7 x8 x9 x10 x11 x12 x13 x14 t.
-       prob_space p ==>
-         (solar_array_FT p x1 x2 x3 x4 x5 x6 x7 x8 x9 x10 x11 x12 x13 x14 t =
-	 rbd_struct p (series (rbd_list (union_unavail_event_list p [x5;x6] t))) UNION
-	 rbd_struct p 
-	   (parallel (rbd_list 
-	   	   (union_unavail_event_list p [x1;x2;x3;x4;x7;x8;x9;x10;x11;x12;x13;x14] t))))``,
-RW_TAC list_ss[solar_array_FT_def,FTree_def,union_unavail_event_list_def,
-	      rbd_struct_def,gate_list_def,rbd_list_def]
-++ SRW_TAC[][UNION_EMPTY,UNION_DEF,INTER_DEF,EXTENSION,GSPECIFICATION]
-++ METIS_TAC[]);
-
-(*-------------------------------------------------*)
-val solar_array_unavail_lemma = store_thm("solar_array_unavail_lemma",
-  ``!p x1 x2 x3 x4 x5 x6 x7 x8 x9 x10 x11 x12 x13 x14 c1 c2 c3 c4 c5 c6 c7 c8 c9 c10 c11 c12 c13 c14 t. 
-  prob_space p /\
-  (!z.  MEM z [c1; c2; c3; c4; c5; c6; c7; c8; c9; c10; c11; c12; c13; c14] ==>
-  	0 < FST z /\ 0 < SND z) /\
-   (∀t'.
-        (∀z.
-           MEM z
-             ((union_unavail_event_list p
-                   [x1; x2; x3; x4; x5; x6; x7; x8; x9; x10; x11; x12; x13; x14]
-                   (&t'))) ⇒
-           z ∈ events p) ∧
-        mutual_indep p
-          ((union_unavail_event_list p
-                [x1; x2; x3; x4; x5; x6; x7; x8; x9; x10; x11; x12; x13; x14]
-                (&t')))) ∧
-     inst_unavail_exp_list p
-       [x1; x2; x3; x4; x5; x6; x7; x8; x9; x10; x11; x12; x13; x14]
-       [c1; c2; c3; c4; c5; c6; c7; c8; c9; c10; c11; c12; c13; c14] ⇒
-       	    (λt.
-   prob p
-     (rbd_struct p
-        (series
-           (rbd_list (union_unavail_event_list p [x5; x6] (&t))))) +
-   prob p
-     (rbd_struct p
-        (parallel
-           (rbd_list
-              (union_unavail_event_list p
-                 [x1; x2; x3; x4; x7; x8; x9; x10; x11; x12; x13; x14]
-                 (&t))))) −
-   prob p
-     (rbd_struct p
-        (series (rbd_list (union_unavail_event_list p [x5; x6] (&t)))) ∩
-      rbd_struct p
-        (series
-           (MAP (λa. parallel (rbd_list a))
-              (list_union_unavail_event_list p
-                 [[x1; x2; x3; x4; x7; x8; x9; x10; x11; x12; x13; x14]]
-                 (&t)))))) -->
-(list_prod (steady_state_unavail_list [c5; c6]) +
- (1 −
-  list_prod
-    (one_minus_list
-       (steady_state_unavail_list
-          [c1; c2; c3; c4; c7; c8; c9; c10; c11; c12; c13; c14]))) −
- list_prod (steady_state_unavail_list [c5; c6]) *
- (1 −
-  list_prod
-    (one_minus_list
-       (steady_state_unavail_list
-          [c1; c2; c3; c4; c7; c8; c9; c10; c11; c12; c13; c14]))))``,
-RW_TAC std_ss[]
-++ (` (λt.
-   prob p
-     (rbd_struct p
-        (series
-           (rbd_list (union_unavail_event_list p [x5; x6] (&t))))) +
-   prob p
-     (rbd_struct p
-        (parallel
-           (rbd_list
-              (union_unavail_event_list p
-                 [x1; x2; x3; x4; x7; x8; x9; x10; x11; x12; x13; x14]
-                 (&t))))) -
-   prob p
-     (rbd_struct p
-        (series (rbd_list (union_unavail_event_list p [x5; x6] (&t)))) ∩
-      rbd_struct p
-        (series
-           (MAP (λa. parallel (rbd_list a))
-              (list_union_unavail_event_list p
-                 [[x1; x2; x3; x4; x7; x8; x9; x10; x11; x12; x13; x14]]
-                 (&t)))))) =
- (\t.
-   (\t.
-     prob p
-     (rbd_struct p
-        (series
-           (rbd_list (union_unavail_event_list p [x5; x6] (&t))))) +
-   prob p
-     (rbd_struct p
-        (parallel
-           (rbd_list
-              (union_unavail_event_list p
-                 [x1; x2; x3; x4; x7; x8; x9; x10; x11; x12; x13; x14]
-                 (&t))))) ) t -
-   (\t.
-     prob p
-     (rbd_struct p
-        (series (rbd_list (union_unavail_event_list p [x5; x6] (&t)))) ∩
-      rbd_struct p
-        (series
-           (MAP (λa. parallel (rbd_list a))
-              (list_union_unavail_event_list p
-                 [[x1; x2; x3; x4; x7; x8; x9; x10; x11; x12; x13; x14]]
-                 (&t)))))) t) ` by RW_TAC real_ss[])
-   ++ POP_ORW
-   ++ MATCH_MP_TAC SEQ_SUB
-   ++ RW_TAC real_ss[]
-   >> ((`(λt.
-   prob p
-     (rbd_struct p
-        (series
-           (rbd_list (union_unavail_event_list p [x5; x6] (&t))))) +
-   prob p
-     (rbd_struct p
-        (parallel
-           (rbd_list
-              (union_unavail_event_list p
-                 [x1; x2; x3; x4; x7; x8; x9; x10; x11; x12; x13; x14]
-                 (&t)))))) =
-     (λt.
-   (\t. prob p
-     (rbd_struct p
-        (series
-           (rbd_list (union_unavail_event_list p [x5; x6] (&t)))))) t +
-  (\t.  prob p
-     (rbd_struct p
-        (parallel
-           (rbd_list
-              (union_unavail_event_list p
-                 [x1; x2; x3; x4; x7; x8; x9; x10; x11; x12; x13; x14]
-                 (&t)))))) t)` by RW_TAC list_ss[])
-      ++ POP_ORW
-      ++ MATCH_MP_TAC SEQ_ADD
-      ++ RW_TAC list_ss[]
-      >> (DEP_REWRITE_TAC[GSYM AND_to_series]
-      	 ++ (`!t.
-       prob p
-       (FTree p
-          (AND (gate_list (union_unavail_event_list p [x5; x6] (&t))))) =
-        list_prod (list_prob p (union_unavail_event_list p [x5; x6] (&t)))` by RW_TAC std_ss[])
-	>> (MATCH_MP_TAC AND_gate_thm
-	   ++ FULL_SIMP_TAC list_ss[union_unavail_event_list_def,rbd_list_def,rbd_struct_def]
-	   ++ STRIP_TAC
-   	   >> (METIS_TAC[])
-	   ++ MATCH_MP_TAC mutual_indep_front_append
-	   ++ EXISTS_TAC(--`[union_unavail_events p x1 (&t);
-           union_unavail_events p x2 (&t);
-           union_unavail_events p x3 (&t);
-           union_unavail_events p x4 (&t)]`--)
-	   ++ MATCH_MP_TAC mutual_indep_flat_append
-	   ++ EXISTS_TAC(--`[[union_unavail_events p x7 (&t);
-           union_unavail_events p x8 (&t);
-           union_unavail_events p x9 (&t);
-           union_unavail_events p x10 (&t);
-           union_unavail_events p x11 (&t);
-           union_unavail_events p x12 (&t);
-           union_unavail_events p x13 (&t);
-           union_unavail_events p x14 (&t)]]`--)
-	   ++ RW_TAC list_ss[])
-	++ POP_ORW
-	++ MATCH_MP_TAC AND_inst_avail_prod_tends_steady
-   	++ FULL_SIMP_TAC list_ss[inst_unavail_exp_list_def]
-	++ METIS_TAC[])
-   ++ DEP_REWRITE_TAC[GSYM OR_to_parallel]
-   ++ (`!t. 
-      	 prob p
-     	  (FTree p
-            (OR
-              (gate_list
-                (union_unavail_event_list p
-                  [x1; x2; x3; x4; x7; x8; x9; x10; x11; x12; x13; x14]
-                    (&t))))) =
-	 1 - list_prod (one_minus_list (list_prob p 
-	  (union_unavail_event_list p  [x1; x2; x3; x4; x7; x8; x9; x10; x11; x12; x13; x14] (&t))))` by RW_TAC std_ss[])
-   >> (MATCH_MP_TAC OR_gate_thm
-      ++ FULL_SIMP_TAC list_ss[union_unavail_event_list_def]
-      ++ STRIP_TAC 
-      >> (METIS_TAC[])
-      ++ (`[union_unavail_events p x1 (&t); union_unavail_events p x2 (&t);
-      	    union_unavail_events p x3 (&t); union_unavail_events p x4 (&t);
-      	    union_unavail_events p x7 (&t); union_unavail_events p x8 (&t);
-      	    union_unavail_events p x9 (&t); union_unavail_events p x10 (&t);
-      	    union_unavail_events p x11 (&t); union_unavail_events p x12 (&t);
-      	    union_unavail_events p x13 (&t); union_unavail_events p x14 (&t)] =
-   	(FLAT ([union_unavail_events p x1 (&t); union_unavail_events p x2 (&t);
-   	        union_unavail_events p x3 (&t); union_unavail_events p x4 (&t)] ::
-   	       [[union_unavail_events p x7 (&t); union_unavail_events p x8 (&t);
-   	         union_unavail_events p x9 (&t); union_unavail_events p x10 (&t);
-   		 union_unavail_events p x11 (&t); union_unavail_events p x12 (&t);
-   		 union_unavail_events p x13 (&t); union_unavail_events p x14 (&t)]]))` by RW_TAC list_ss[])
-     ++ POP_ORW
-     ++ MATCH_MP_TAC mutual_indep_flat_cons3
-     ++ EXISTS_TAC (--`[union_unavail_events p x5 (&t);union_unavail_events p x6 (&t)]`--)
-     ++ RW_TAC list_ss[])
-  ++ POP_ORW
-  ++ (`(\t.
-   1 −
-   list_prod
-     (one_minus_list
-        (list_prob p 
-	 (union_unavail_event_list p [x1; x2; x3; x4; x7; x8; x9; x10; x11; x12; x13; x14] (&t))))) = 
-  (\t.
-   (\t. 1) t −
-   (\t. list_prod
-     (one_minus_list
-        (list_prob p 
-	 (union_unavail_event_list p [x1; x2; x3; x4; x7; x8; x9; x10; x11; x12; x13; x14] (&t))))) t) ` by RW_TAC real_ss[])
-   ++ POP_ORW
-   ++ MATCH_MP_TAC SEQ_SUB
-   ++ RW_TAC std_ss[SEQ_CONST]
-  ++ MATCH_MP_TAC lim_inst_OR_tend_steady
-   ++ FULL_SIMP_TAC list_ss[inst_unavail_exp_list_def]
-   ++ METIS_TAC[])
-++ (`(!t. 
-      prob p
-     (rbd_struct p
-        (series (rbd_list (union_unavail_event_list p [x5; x6] (&t)))) ∩
-      rbd_struct p
-        (series
-           (MAP (λa. parallel (rbd_list a))
-              (list_union_unavail_event_list p
-                 [[x1; x2; x3; x4; x7; x8; x9; x10; x11; x12; x13; x14]]
-                 (&t))))) =
-   prob p
-     (rbd_struct p
-        (series (rbd_list (union_unavail_event_list p [x5; x6] (&t))))) *
-   prob p (rbd_struct p
-        (series
-           (MAP (λa. parallel (rbd_list a))
-              (list_union_unavail_event_list p
-                 [[x1; x2; x3; x4; x7; x8; x9; x10; x11; x12; x13; x14]]
-                 (&t))))))` by RW_TAC std_ss[])
-   >> (DEP_REWRITE_TAC [series_rbd_indep_series_parallel_rbd]
-      ++ FULL_SIMP_TAC list_ss[union_unavail_event_list_def,list_union_unavail_event_list_def]
-      ++ STRIP_TAC
-      >> (METIS_TAC[NULL])
-      ++ STRIP_TAC
-      >> (METIS_TAC[NULL])
-      ++ (`[union_unavail_events p x5 (&t); union_unavail_events p x6 (&t);
-   union_unavail_events p x1 (&t); union_unavail_events p x2 (&t);
-   union_unavail_events p x3 (&t); union_unavail_events p x4 (&t);
-   union_unavail_events p x7 (&t); union_unavail_events p x8 (&t);
-   union_unavail_events p x9 (&t); union_unavail_events p x10 (&t);
-   union_unavail_events p x11 (&t); union_unavail_events p x12 (&t);
-   union_unavail_events p x13 (&t); union_unavail_events p x14 (&t)] =
-   	 [union_unavail_events p x5 (&t); union_unavail_events p x6 (&t)] ++
-   [union_unavail_events p x1 (&t); union_unavail_events p x2 (&t);
-   union_unavail_events p x3 (&t); union_unavail_events p x4 (&t)] ++
-   [union_unavail_events p x7 (&t); union_unavail_events p x8 (&t);
-   union_unavail_events p x9 (&t); union_unavail_events p x10 (&t);
-   union_unavail_events p x11 (&t); union_unavail_events p x12 (&t);
-   union_unavail_events p x13 (&t); union_unavail_events p x14 (&t)]` by RW_TAC list_ss[])
-      ++ POP_ORW
-      ++ MATCH_MP_TAC mutual_indep_append1
-      ++ RW_TAC list_ss[])
-  ++ POP_ORW
-  ++ (`!t. 
-     	(λt.
-   prob p
-     (rbd_struct p
-        (series
-           (rbd_list (union_unavail_event_list p [x5; x6] (&t))))) *
-   prob p
-     (rbd_struct p
-        (series
-           (MAP (λa. parallel (rbd_list a))
-              (list_union_unavail_event_list p
-                 [[x1; x2; x3; x4; x7; x8; x9; x10; x11; x12; x13; x14]]
-                 (&t)))))) =
-      (λt.
-   (\t. prob p
-     (rbd_struct p
-        (series
-           (rbd_list (union_unavail_event_list p [x5; x6] (&t)))))) t *
-   (\t. prob p
-     (rbd_struct p
-        (series
-           (MAP (λa. parallel (rbd_list a))
-              (list_union_unavail_event_list p
-                 [[x1; x2; x3; x4; x7; x8; x9; x10; x11; x12; x13; x14]]
-                 (&t)))))) t)` by RW_TAC list_ss[])
-  ++ POP_ORW
-  ++ MATCH_MP_TAC SEQ_MUL
-  ++ RW_TAC std_ss[]
-  >> (DEP_REWRITE_TAC[GSYM AND_to_series]
-      	 ++ (`!t.
-       prob p
-       (FTree p
-          (AND (gate_list (union_unavail_event_list p [x5; x6] (&t))))) =
-        list_prod (list_prob p (union_unavail_event_list p [x5; x6] (&t)))` by RW_TAC std_ss[])
-	>> (MATCH_MP_TAC AND_gate_thm
-	   ++ FULL_SIMP_TAC list_ss[union_unavail_event_list_def,rbd_list_def,rbd_struct_def]
-	   ++ STRIP_TAC
-   	   >> (METIS_TAC[])
-	   ++ MATCH_MP_TAC mutual_indep_front_append
-	   ++ EXISTS_TAC(--`[union_unavail_events p x1 (&t);
-           union_unavail_events p x2 (&t);
-           union_unavail_events p x3 (&t);
-           union_unavail_events p x4 (&t)]`--)
-	   ++ MATCH_MP_TAC mutual_indep_flat_append
-	   ++ EXISTS_TAC(--`[[union_unavail_events p x7 (&t);
-           union_unavail_events p x8 (&t);
-           union_unavail_events p x9 (&t);
-           union_unavail_events p x10 (&t);
-           union_unavail_events p x11 (&t);
-           union_unavail_events p x12 (&t);
-           union_unavail_events p x13 (&t);
-           union_unavail_events p x14 (&t)]]`--)
-	   ++ RW_TAC list_ss[])
-	++ POP_ORW
-	++ MATCH_MP_TAC AND_inst_avail_prod_tends_steady
-   	++ FULL_SIMP_TAC list_ss[inst_unavail_exp_list_def]
-	++ METIS_TAC[])
-  ++ (`!t. 
-     	(rbd_struct p
-	  (series (MAP (λa. parallel (rbd_list a))
-	    (list_union_unavail_event_list p
-                   [[x1; x2; x3; x4; x7; x8; x9; x10; x11; x12; x13; x14]]
-                   (&t))))) = 
-	(rbd_struct p 
-             (parallel (rbd_list
-	     	   (union_unavail_event_list p [x1;x2;x3;x4;x7;x8;x9;x10;x11;x12;x13;x14] (&t)))))`
-		   by RW_TAC list_ss[rbd_list_def,list_union_unavail_event_list_def,union_unavail_event_list_def,rbd_struct_def,UNION_EMPTY])
-  >> (ONCE_REWRITE_TAC[INTER_COMM]
-     ++ DEP_REWRITE_TAC[INTER_PSPACE]
-     ++ FULL_SIMP_TAC list_ss[union_unavail_event_list_def]
-     ++ DEP_REWRITE_TAC[EVENTS_UNION]
-     ++ METIS_TAC[])
-  ++ POP_ORW
-  ++ DEP_REWRITE_TAC[GSYM OR_to_parallel]
-   ++ (`!t. 
-      	 prob p
-     	  (FTree p
-            (OR
-              (gate_list
-                (union_unavail_event_list p
-                  [x1; x2; x3; x4; x7; x8; x9; x10; x11; x12; x13; x14]
-                    (&t))))) =
-	 1 - list_prod (one_minus_list (list_prob p 
-	  (union_unavail_event_list p  [x1; x2; x3; x4; x7; x8; x9; x10; x11; x12; x13; x14] (&t))))` by RW_TAC std_ss[])
-   >> (MATCH_MP_TAC OR_gate_thm
-      ++ FULL_SIMP_TAC list_ss[union_unavail_event_list_def]
-      ++ STRIP_TAC 
-      >> (METIS_TAC[])
-      ++ (`[union_unavail_events p x1 (&t); union_unavail_events p x2 (&t);
-      	    union_unavail_events p x3 (&t); union_unavail_events p x4 (&t);
-      	    union_unavail_events p x7 (&t); union_unavail_events p x8 (&t);
-      	    union_unavail_events p x9 (&t); union_unavail_events p x10 (&t);
-      	    union_unavail_events p x11 (&t); union_unavail_events p x12 (&t);
-      	    union_unavail_events p x13 (&t); union_unavail_events p x14 (&t)] =
-   	(FLAT ([union_unavail_events p x1 (&t); union_unavail_events p x2 (&t);
-   	        union_unavail_events p x3 (&t); union_unavail_events p x4 (&t)] ::
-   	       [[union_unavail_events p x7 (&t); union_unavail_events p x8 (&t);
-   	         union_unavail_events p x9 (&t); union_unavail_events p x10 (&t);
-   		 union_unavail_events p x11 (&t); union_unavail_events p x12 (&t);
-   		 union_unavail_events p x13 (&t); union_unavail_events p x14 (&t)]]))` by RW_TAC list_ss[])
-     ++ POP_ORW
-     ++ MATCH_MP_TAC mutual_indep_flat_cons3
-     ++ EXISTS_TAC (--`[union_unavail_events p x5 (&t);union_unavail_events p x6 (&t)]`--)
-     ++ RW_TAC list_ss[])
-  ++ POP_ORW
-  ++ (`(\t.
-   1 −
-   list_prod
-     (one_minus_list
-        (list_prob p (union_unavail_event_list p [x1; x2; x3; x4; x7; x8; x9; x10; x11; x12; x13; x14] (&t))))) = (\t.
-   (\t. 1) t −
-   (\t. list_prod
-     (one_minus_list
-        (list_prob p (union_unavail_event_list p [x1; x2; x3; x4; x7; x8; x9; x10; x11; x12; x13; x14] (&t))))) t) ` by RW_TAC real_ss[])
-   ++ POP_ORW
-   ++ MATCH_MP_TAC SEQ_SUB
-   ++ RW_TAC std_ss[SEQ_CONST]
-   ++ MATCH_MP_TAC lim_inst_OR_tend_steady
-   ++ FULL_SIMP_TAC list_ss[inst_unavail_exp_list_def]
-   ++ METIS_TAC[]);
-(*-------------------------------------------------*)
-val solar_array_unavail = store_thm("solar_array_unavail",
-  ``!p x1 x2 x3 x4 x5 x6 x7 x8 x9 x10 x11 x12 x13 x14 c1 c2 c3 c4 c5 c6 c7 c8 c9 c10 c11 c12 c13 c14 t. 
-  prob_space p /\
-  (!z.  MEM z [c1; c2; c3; c4; c5; c6; c7; c8; c9; c10; c11; c12; c13; c14] ==>
-  	0 < FST z /\ 0 < SND z) /\
-   (∀t'.
-        (∀z.
-           MEM z
-             ((union_unavail_event_list p
-                   [x1; x2; x3; x4; x5; x6; x7; x8; x9; x10; x11; x12; x13; x14]
-                   (&t'))) ⇒
-           z ∈ events p) ∧
-        mutual_indep p
-          ((union_unavail_event_list p
-                [x1; x2; x3; x4; x5; x6; x7; x8; x9; x10; x11; x12; x13; x14]
-                (&t')))) ∧
-     inst_unavail_exp_list p
-       [x1; x2; x3; x4; x5; x6; x7; x8; x9; x10; x11; x12; x13; x14]
-       [c1; c2; c3; c4; c5; c6; c7; c8; c9; c10; c11; c12; c13; c14] ⇒
-
-       (lim
-        (λt.
-           prob p
-            (rbd_struct p (series (rbd_list (union_unavail_event_list p [x5;x6] (&t)))) UNION
-	     rbd_struct p
-	      (parallel (rbd_list
-	      	 (union_unavail_event_list p [x1;x2;x3;x4;x7;x8;x9;x10;x11;x12;x13;x14] (&t)))))) =
-       list_prod (steady_state_unavail_list [c5;c6]) +
-       (1 − list_prod (one_minus_list
-       	   (steady_state_unavail_list [c1;c2;c3;c4;c7;c8;c9;c10;c11;c12;c13;c14]))) -
-       (list_prod (steady_state_unavail_list [c5;c6]) * 
-       (1 − list_prod (one_minus_list
-          (steady_state_unavail_list [c1;c2;c3;c4;c7;c8;c9;c10;c11;c12;c13;c14])))))``,
-RW_TAC std_ss[]
-++ (`!t. 
-       prob p
-         (rbd_struct p 
-	    (series (rbd_list (union_unavail_event_list p [x5;x6] (&t)))) UNION
-	  rbd_struct p 
-	    (parallel (rbd_list 
-	      (union_unavail_event_list p [x1;x2;x3;x4;x7;x8;x9;x10;x11;x12;x13;x14] (&t))))) =  
-       prob p
-         (rbd_struct p (series (rbd_list (union_unavail_event_list p [x5;x6] (&t))))) + 
-       prob p 
-         (rbd_struct p 
-	    (parallel (rbd_list 
-               (union_unavail_event_list p [x1;x2;x3;x4;x7;x8;x9;x10;x11;x12;x13;x14] (&t))))) - 
-       prob p
-         (rbd_struct p (series (rbd_list (union_unavail_event_list p [x5;x6] (&t)))) INTER
-	  rbd_struct p 
-             (parallel (rbd_list
-	     	   (union_unavail_event_list p [x1;x2;x3;x4;x7;x8;x9;x10;x11;x12;x13;x14] (&t)))))` by RW_TAC std_ss[])
->> (MATCH_MP_TAC Prob_Incl_excl
-   ++ RW_TAC list_ss[]
-   >> (RW_TAC std_ss[series_rbd_eq_big_inter]
-      ++ MATCH_MP_TAC in_events_big_inter
-      ++ FULL_SIMP_TAC list_ss[union_unavail_event_list_def]
-      ++ METIS_TAC[])
-   ++ FULL_SIMP_TAC list_ss[union_unavail_event_list_def,rbd_list_def,rbd_struct_def,UNION_EMPTY]
-   ++ DEP_REWRITE_TAC[EVENTS_UNION]
-   ++ METIS_TAC[])
-++ POP_ORW
-++ (`(!t. (rbd_struct p
-          (series
-             (rbd_list (union_unavail_event_list p [x5; x6] (&t)))) ∩
-        rbd_struct p
-          (parallel
-             (rbd_list
-                (union_unavail_event_list p
-                   [x1; x2; x3; x4; x7; x8; x9; x10; x11; x12; x13; x14]
-                   (&t))))) =
-    (rbd_struct p
-          (series
-             (rbd_list (union_unavail_event_list p [x5; x6] (&t)))) ∩
-        rbd_struct p (series (MAP (λa. parallel (rbd_list a)) (list_union_unavail_event_list p
-                   [[x1; x2; x3; x4; x7; x8; x9; x10; x11; x12; x13; x14]]
-                   (&t))))))` by RW_TAC std_ss[])
->> (RW_TAC list_ss[rbd_list_def,rbd_struct_def,list_union_unavail_event_list_def,union_unavail_event_list_def,UNION_EMPTY]
-   ++ SRW_TAC [][EXTENSION,GSPECIFICATION,UNION_DEF]
-   ++ METIS_TAC[])
-++ POP_ORW
-++ MATCH_MP_TAC SEQ_UNIQ
-++ EXISTS_TAC(--`(λt.
-       prob p
-         (rbd_struct p
-            (series
-               (rbd_list (union_unavail_event_list p [x5; x6] (&t))))) +
-       prob p
-         (rbd_struct p
-            (parallel
-               (rbd_list
-                  (union_unavail_event_list p
-                     [x1; x2; x3; x4; x7; x8; x9; x10; x11; x12; x13;
-                      x14] (&t))))) −
-       prob p
-         (rbd_struct p
-            (series
-               (rbd_list (union_unavail_event_list p [x5; x6] (&t)))) ∩
-          rbd_struct p
-            (series
-               (MAP (λa. parallel (rbd_list a))
-                  (list_union_unavail_event_list p
-                     [[x1; x2; x3; x4; x7; x8; x9; x10; x11; x12; x13;
-                       x14]] (&t))))))`--)
-++ RW_TAC std_ss[GSYM SEQ_LIM,convergent]
->> (EXISTS_TAC(--`
-list_prod (steady_state_unavail_list [c5;c6]) +
-       (1 − list_prod (one_minus_list
-       	   (steady_state_unavail_list [c1;c2;c3;c4;c7;c8;c9;c10;c11;c12;c13;c14]))) -
-       (list_prod (steady_state_unavail_list [c5;c6]) * 
-       (1 − list_prod (one_minus_list
-          (steady_state_unavail_list [c1;c2;c3;c4;c7;c8;c9;c10;c11;c12;c13;c14]))))`--)
-   ++ (` (λt.
-   prob p
-     (rbd_struct p
-        (series
-           (rbd_list (union_unavail_event_list p [x5; x6] (&t))))) +
-   prob p
-     (rbd_struct p
-        (parallel
-           (rbd_list
-              (union_unavail_event_list p
-                 [x1; x2; x3; x4; x7; x8; x9; x10; x11; x12; x13; x14]
-                 (&t))))) -
-   prob p
-     (rbd_struct p
-        (series (rbd_list (union_unavail_event_list p [x5; x6] (&t)))) ∩
-      rbd_struct p
-        (series
-           (MAP (λa. parallel (rbd_list a))
-              (list_union_unavail_event_list p
-                 [[x1; x2; x3; x4; x7; x8; x9; x10; x11; x12; x13; x14]]
-                 (&t)))))) =
- (\t.
-   (\t.
-     prob p
-     (rbd_struct p
-        (series
-           (rbd_list (union_unavail_event_list p [x5; x6] (&t))))) +
-   prob p
-     (rbd_struct p
-        (parallel
-           (rbd_list
-              (union_unavail_event_list p
-                 [x1; x2; x3; x4; x7; x8; x9; x10; x11; x12; x13; x14]
-                 (&t))))) ) t -
-   (\t.
-     prob p
-     (rbd_struct p
-        (series (rbd_list (union_unavail_event_list p [x5; x6] (&t)))) ∩
-      rbd_struct p
-        (series
-           (MAP (λa. parallel (rbd_list a))
-              (list_union_unavail_event_list p
-                 [[x1; x2; x3; x4; x7; x8; x9; x10; x11; x12; x13; x14]]
-                 (&t)))))) t) ` by RW_TAC real_ss[])
-   ++ POP_ORW
-   ++ MATCH_MP_TAC SEQ_SUB
-   ++ RW_TAC real_ss[]
-   >> ((`(λt.
-   prob p
-     (rbd_struct p
-        (series
-           (rbd_list (union_unavail_event_list p [x5; x6] (&t))))) +
-   prob p
-     (rbd_struct p
-        (parallel
-           (rbd_list
-              (union_unavail_event_list p
-                 [x1; x2; x3; x4; x7; x8; x9; x10; x11; x12; x13; x14]
-                 (&t)))))) =
-     (λt.
-   (\t. prob p
-     (rbd_struct p
-        (series
-           (rbd_list (union_unavail_event_list p [x5; x6] (&t)))))) t +
-  (\t.  prob p
-     (rbd_struct p
-        (parallel
-           (rbd_list
-              (union_unavail_event_list p
-                 [x1; x2; x3; x4; x7; x8; x9; x10; x11; x12; x13; x14]
-                 (&t)))))) t)` by RW_TAC list_ss[])
-      ++ POP_ORW
-      ++ MATCH_MP_TAC SEQ_ADD
-      ++ RW_TAC list_ss[]
-      >> (DEP_REWRITE_TAC[GSYM AND_to_series]
-      	 ++ (`!t.
-       prob p
-       (FTree p
-          (AND (gate_list (union_unavail_event_list p [x5; x6] (&t))))) =
-        list_prod (list_prob p (union_unavail_event_list p [x5; x6] (&t)))` by RW_TAC std_ss[])
-	>> (MATCH_MP_TAC AND_gate_thm
-	   ++ FULL_SIMP_TAC list_ss[union_unavail_event_list_def,rbd_list_def,rbd_struct_def]
-	   ++ STRIP_TAC
-   	   >> (METIS_TAC[])
-	   ++ MATCH_MP_TAC mutual_indep_front_append
-	   ++ EXISTS_TAC(--`[union_unavail_events p x1 (&t);
-           union_unavail_events p x2 (&t);
-           union_unavail_events p x3 (&t);
-           union_unavail_events p x4 (&t)]`--)
-	   ++ MATCH_MP_TAC mutual_indep_flat_append
-	   ++ EXISTS_TAC(--`[[union_unavail_events p x7 (&t);
-           union_unavail_events p x8 (&t);
-           union_unavail_events p x9 (&t);
-           union_unavail_events p x10 (&t);
-           union_unavail_events p x11 (&t);
-           union_unavail_events p x12 (&t);
-           union_unavail_events p x13 (&t);
-           union_unavail_events p x14 (&t)]]`--)
-	   ++ RW_TAC list_ss[])
-	++ POP_ORW
-	++ MATCH_MP_TAC AND_inst_avail_prod_tends_steady
-   	++ FULL_SIMP_TAC list_ss[inst_unavail_exp_list_def]
-	++ METIS_TAC[])
-   ++ DEP_REWRITE_TAC[GSYM OR_to_parallel]
-   ++ (`!t. 
-      	 prob p
-     	  (FTree p
-            (OR
-              (gate_list
-                (union_unavail_event_list p
-                  [x1; x2; x3; x4; x7; x8; x9; x10; x11; x12; x13; x14]
-                    (&t))))) =
-	 1 - list_prod (one_minus_list (list_prob p 
-	  (union_unavail_event_list p  [x1; x2; x3; x4; x7; x8; x9; x10; x11; x12; x13; x14] (&t))))` by RW_TAC std_ss[])
-   >> (MATCH_MP_TAC OR_gate_thm
-      ++ FULL_SIMP_TAC list_ss[union_unavail_event_list_def]
-      ++ STRIP_TAC 
-      >> (METIS_TAC[])
-      ++ (`[union_unavail_events p x1 (&t); union_unavail_events p x2 (&t);
-      	    union_unavail_events p x3 (&t); union_unavail_events p x4 (&t);
-      	    union_unavail_events p x7 (&t); union_unavail_events p x8 (&t);
-      	    union_unavail_events p x9 (&t); union_unavail_events p x10 (&t);
-      	    union_unavail_events p x11 (&t); union_unavail_events p x12 (&t);
-      	    union_unavail_events p x13 (&t); union_unavail_events p x14 (&t)] =
-   	(FLAT ([union_unavail_events p x1 (&t); union_unavail_events p x2 (&t);
-   	        union_unavail_events p x3 (&t); union_unavail_events p x4 (&t)] ::
-   	       [[union_unavail_events p x7 (&t); union_unavail_events p x8 (&t);
-   	         union_unavail_events p x9 (&t); union_unavail_events p x10 (&t);
-   		 union_unavail_events p x11 (&t); union_unavail_events p x12 (&t);
-   		 union_unavail_events p x13 (&t); union_unavail_events p x14 (&t)]]))` by RW_TAC list_ss[])
-     ++ POP_ORW
-     ++ MATCH_MP_TAC mutual_indep_flat_cons3
-     ++ EXISTS_TAC (--`[union_unavail_events p x5 (&t);union_unavail_events p x6 (&t)]`--)
-     ++ RW_TAC list_ss[])
-  ++ POP_ORW
-  ++ (`(\t.
-   1 −
-   list_prod
-     (one_minus_list
-        (list_prob p (union_unavail_event_list p [x1; x2; x3; x4; x7; x8; x9; x10; x11; x12; x13; x14] (&t))))) = (\t.
-   (\t. 1) t −
-   (\t. list_prod
-     (one_minus_list
-        (list_prob p (union_unavail_event_list p [x1; x2; x3; x4; x7; x8; x9; x10; x11; x12; x13; x14] (&t))))) t) ` by RW_TAC real_ss[])
-   ++ POP_ORW
-   ++ MATCH_MP_TAC SEQ_SUB
-   ++ RW_TAC std_ss[SEQ_CONST]
-  ++ MATCH_MP_TAC lim_inst_OR_tend_steady
-   ++ FULL_SIMP_TAC list_ss[inst_unavail_exp_list_def]
-   ++ METIS_TAC[])
-++ (`(!t. 
-      prob p
-     (rbd_struct p
-        (series (rbd_list (union_unavail_event_list p [x5; x6] (&t)))) ∩
-      rbd_struct p
-        (series
-           (MAP (λa. parallel (rbd_list a))
-              (list_union_unavail_event_list p
-                 [[x1; x2; x3; x4; x7; x8; x9; x10; x11; x12; x13; x14]]
-                 (&t))))) =
-   prob p
-     (rbd_struct p
-        (series (rbd_list (union_unavail_event_list p [x5; x6] (&t))))) *
-   prob p (rbd_struct p
-        (series
-           (MAP (λa. parallel (rbd_list a))
-              (list_union_unavail_event_list p
-                 [[x1; x2; x3; x4; x7; x8; x9; x10; x11; x12; x13; x14]]
-                 (&t))))))` by RW_TAC std_ss[])
-   >> (DEP_REWRITE_TAC [series_rbd_indep_series_parallel_rbd]
-      ++ FULL_SIMP_TAC list_ss[union_unavail_event_list_def,list_union_unavail_event_list_def]
-      ++ STRIP_TAC
-      >> (METIS_TAC[NULL])
-      ++ STRIP_TAC
-      >> (METIS_TAC[NULL])
-      ++ (`[union_unavail_events p x5 (&t); union_unavail_events p x6 (&t);
-   union_unavail_events p x1 (&t); union_unavail_events p x2 (&t);
-   union_unavail_events p x3 (&t); union_unavail_events p x4 (&t);
-   union_unavail_events p x7 (&t); union_unavail_events p x8 (&t);
-   union_unavail_events p x9 (&t); union_unavail_events p x10 (&t);
-   union_unavail_events p x11 (&t); union_unavail_events p x12 (&t);
-   union_unavail_events p x13 (&t); union_unavail_events p x14 (&t)] =
-   	 [union_unavail_events p x5 (&t); union_unavail_events p x6 (&t)] ++
-   [union_unavail_events p x1 (&t); union_unavail_events p x2 (&t);
-   union_unavail_events p x3 (&t); union_unavail_events p x4 (&t)] ++
-   [union_unavail_events p x7 (&t); union_unavail_events p x8 (&t);
-   union_unavail_events p x9 (&t); union_unavail_events p x10 (&t);
-   union_unavail_events p x11 (&t); union_unavail_events p x12 (&t);
-   union_unavail_events p x13 (&t); union_unavail_events p x14 (&t)]` by RW_TAC list_ss[])
-      ++ POP_ORW
-      ++ MATCH_MP_TAC mutual_indep_append1
-      ++ RW_TAC list_ss[])
-  ++ POP_ORW
-  ++ (`!t. 
-     	(λt.
-   prob p
-     (rbd_struct p
-        (series
-           (rbd_list (union_unavail_event_list p [x5; x6] (&t))))) *
-   prob p
-     (rbd_struct p
-        (series
-           (MAP (λa. parallel (rbd_list a))
-              (list_union_unavail_event_list p
-                 [[x1; x2; x3; x4; x7; x8; x9; x10; x11; x12; x13; x14]]
-                 (&t)))))) =
-      (λt.
-   (\t. prob p
-     (rbd_struct p
-        (series
-           (rbd_list (union_unavail_event_list p [x5; x6] (&t)))))) t *
-   (\t. prob p
-     (rbd_struct p
-        (series
-           (MAP (λa. parallel (rbd_list a))
-              (list_union_unavail_event_list p
-                 [[x1; x2; x3; x4; x7; x8; x9; x10; x11; x12; x13; x14]]
-                 (&t)))))) t)` by RW_TAC list_ss[])
-  ++ POP_ORW
-  ++ MATCH_MP_TAC SEQ_MUL
-  ++ RW_TAC std_ss[]
-  >> (DEP_REWRITE_TAC[GSYM AND_to_series]
-      	 ++ (`!t.
-       prob p
-       (FTree p
-          (AND (gate_list (union_unavail_event_list p [x5; x6] (&t))))) =
-        list_prod (list_prob p (union_unavail_event_list p [x5; x6] (&t)))` by RW_TAC std_ss[])
-	>> (MATCH_MP_TAC AND_gate_thm
-	   ++ FULL_SIMP_TAC list_ss[union_unavail_event_list_def,rbd_list_def,rbd_struct_def]
-	   ++ STRIP_TAC
-   	   >> (METIS_TAC[])
-	   ++ MATCH_MP_TAC mutual_indep_front_append
-	   ++ EXISTS_TAC(--`[union_unavail_events p x1 (&t);
-           union_unavail_events p x2 (&t);
-           union_unavail_events p x3 (&t);
-           union_unavail_events p x4 (&t)]`--)
-	   ++ MATCH_MP_TAC mutual_indep_flat_append
-	   ++ EXISTS_TAC(--`[[union_unavail_events p x7 (&t);
-           union_unavail_events p x8 (&t);
-           union_unavail_events p x9 (&t);
-           union_unavail_events p x10 (&t);
-           union_unavail_events p x11 (&t);
-           union_unavail_events p x12 (&t);
-           union_unavail_events p x13 (&t);
-           union_unavail_events p x14 (&t)]]`--)
-	   ++ RW_TAC list_ss[])
-	++ POP_ORW
-	++ MATCH_MP_TAC AND_inst_avail_prod_tends_steady
-   	++ FULL_SIMP_TAC list_ss[inst_unavail_exp_list_def]
-	++ METIS_TAC[])
-  ++ (`!t. 
-     	(rbd_struct p
-	  (series (MAP (λa. parallel (rbd_list a))
-	    (list_union_unavail_event_list p
-                   [[x1; x2; x3; x4; x7; x8; x9; x10; x11; x12; x13; x14]]
-                   (&t))))) = 
-	(rbd_struct p 
-             (parallel (rbd_list
-	     	   (union_unavail_event_list p [x1;x2;x3;x4;x7;x8;x9;x10;x11;x12;x13;x14] (&t)))))`
-		   by RW_TAC list_ss[rbd_list_def,list_union_unavail_event_list_def,union_unavail_event_list_def,rbd_struct_def,UNION_EMPTY])
-  >> (ONCE_REWRITE_TAC[INTER_COMM]
-     ++ DEP_REWRITE_TAC[INTER_PSPACE]
-     ++ FULL_SIMP_TAC list_ss[union_unavail_event_list_def]
-     ++ DEP_REWRITE_TAC[EVENTS_UNION]
-     ++ METIS_TAC[])
-  ++ POP_ORW
-  ++ DEP_REWRITE_TAC[GSYM OR_to_parallel]
-   ++ (`!t. 
-      	 prob p
-     	  (FTree p
-            (OR
-              (gate_list
-                (union_unavail_event_list p
-                  [x1; x2; x3; x4; x7; x8; x9; x10; x11; x12; x13; x14]
-                    (&t))))) =
-	 1 - list_prod (one_minus_list (list_prob p 
-	  (union_unavail_event_list p  [x1; x2; x3; x4; x7; x8; x9; x10; x11; x12; x13; x14] (&t))))` by RW_TAC std_ss[])
-   >> (MATCH_MP_TAC OR_gate_thm
-      ++ FULL_SIMP_TAC list_ss[union_unavail_event_list_def]
-      ++ STRIP_TAC 
-      >> (METIS_TAC[])
-      ++ (`[union_unavail_events p x1 (&t); union_unavail_events p x2 (&t);
-      	    union_unavail_events p x3 (&t); union_unavail_events p x4 (&t);
-      	    union_unavail_events p x7 (&t); union_unavail_events p x8 (&t);
-      	    union_unavail_events p x9 (&t); union_unavail_events p x10 (&t);
-      	    union_unavail_events p x11 (&t); union_unavail_events p x12 (&t);
-      	    union_unavail_events p x13 (&t); union_unavail_events p x14 (&t)] =
-   	(FLAT ([union_unavail_events p x1 (&t); union_unavail_events p x2 (&t);
-   	        union_unavail_events p x3 (&t); union_unavail_events p x4 (&t)] ::
-   	       [[union_unavail_events p x7 (&t); union_unavail_events p x8 (&t);
-   	         union_unavail_events p x9 (&t); union_unavail_events p x10 (&t);
-   		 union_unavail_events p x11 (&t); union_unavail_events p x12 (&t);
-   		 union_unavail_events p x13 (&t); union_unavail_events p x14 (&t)]]))` by RW_TAC list_ss[])
-     ++ POP_ORW
-     ++ MATCH_MP_TAC mutual_indep_flat_cons3
-     ++ EXISTS_TAC (--`[union_unavail_events p x5 (&t);union_unavail_events p x6 (&t)]`--)
-     ++ RW_TAC list_ss[])
-  ++ POP_ORW
-  ++ (`(\t.
-   1 −
-   list_prod
-     (one_minus_list
-        (list_prob p (union_unavail_event_list p [x1; x2; x3; x4; x7; x8; x9; x10; x11; x12; x13; x14] (&t))))) = (\t.
-   (\t. 1) t −
-   (\t. list_prod
-     (one_minus_list
-        (list_prob p (union_unavail_event_list p [x1; x2; x3; x4; x7; x8; x9; x10; x11; x12; x13; x14] (&t))))) t) ` by RW_TAC real_ss[])
-   ++ POP_ORW
-   ++ MATCH_MP_TAC SEQ_SUB
-   ++ RW_TAC std_ss[SEQ_CONST]
-  ++ MATCH_MP_TAC lim_inst_OR_tend_steady
-   ++ FULL_SIMP_TAC list_ss[inst_unavail_exp_list_def]
-   ++ METIS_TAC[])
-++ MATCH_MP_TAC solar_array_unavail_lemma
-++ RW_TAC std_ss[]
-++ METIS_TAC[union_unavail_event_list_def]);
-
 val _ = export_theory();
